\documentclass{article}
\makeatletter
\newcommand*{\rom}[1]{\expandafter\@slowromancap\romannumeral #1@}
\makeatother
\usepackage{amsfonts, amssymb}
\usepackage{mathrsfs, mathdots} 
\usepackage{amsmath}
\usepackage{float}
\usepackage{amsthm}
\usepackage{tikz-cd}
\usepackage{xcolor}
\usepackage{xparse}
\usepackage{setspace}
\usepackage{xfrac}
\usepackage{yfonts}
\setcounter{MaxMatrixCols}{11}

\newtheorem{theorem}{Theorem}[subsection]
\newtheorem{proposition}[theorem]{Proposition}
\newtheorem{corollary}[theorem]{Corollary}
\newtheorem{lemma}[theorem]{Lemma}
\newtheorem{notations}[theorem]{Notations}
\newtheorem{definition}[theorem]{Definition}
\newtheorem{example}[theorem]{Example}
\newtheorem{remark}[theorem]{Remark}

\newtheorem{theorem2}{Theorem}[section]
\newtheorem{proposition2}[theorem2]{Proposition}
\newtheorem{corollary2}[theorem2]{Corollary}
\newtheorem{lemma2}[theorem2]{Lemma}
\newtheorem{notations2}[theorem2]{Notations}
\newtheorem{definition2}[theorem2]{Definition}
\newtheorem{example2}[theorem2]{Example}
\newtheorem{remark2}[theorem2]{Remark}

\ExplSyntaxOn
\NewDocumentCommand{\cycle}{ O{\;} m }
 {
  (
  \alec_cycle:nn { #1 } { #2 }
  )
 }

\seq_new:N \l_alec_cycle_seq
\cs_new_protected:Npn \alec_cycle:nn #1 #2
 {
  \seq_set_split:Nnn \l_alec_cycle_seq { , } { #2 }
  \seq_use:Nn \l_alec_cycle_seq { #1 }
 }
\ExplSyntaxOff
\usepackage{titling}
\newcommand{\subtitle}[1]{%
  \posttitle{%
    \par\end{center}
    \begin{center}\large#1\end{center}
    \vskip0.5em}%
}
\usepackage{arydshln}
\setcounter{tocdepth}{2}
\setlength{\dashlinedash}{1.2pt}
\setlength{\dashlinegap}{1.5pt}
\setlength{\arrayrulewidth}{0.2pt}
\usepackage{graphicx} % Required for inserting images

\begin{document}
\section{The computation of $G_{n}(\mathbb{Z}_{p})$}
\begin{proposition2}
Define $\eta:\mathcal{L}_{n,p}\rightarrow\mathcal{L}_{n,p}$ by \[\eta(e_{ij}):=(-1)^{j-i-1}e_{n+1-j,n+1-i},\]\\ for all $1\leq{i}<{j}\leq{n}$. Then
$\eta\in{G_{n}(\mathbb{Q}_{p})}$.
\end{proposition2}
\begin{proof}
Let $e_{ij},e_{jk}\in\mathcal{L}_{n,p}$, then $\eta([e_{ij},e_{jk}])=\eta(e_{ik})=(-1)^{k-i-1}e_{n+1-k,n+1-i}=(-1)^{k-j+j-i-1}[e_{n+1-k,n+1-j},e_{n+1-j,n+1-i}]=$\[=[(-1)^{k-j}e_{n+1-k,n+1-j},(-1)^{j-i-1}e_{n+1-j,n+1-i}]=\]\[=-[(-1)^{k-j-1}e_{n+1-k,n+1-j},(-1)^{j-i-1}e_{n+1-j,n+1-i}]=\]\[=-[\eta(e_{jk}),\eta(e_{ij})]=[\eta(e_{ij}),\eta(e_{jk})].\]
Therefore $\eta$ is compatible with the Lie bracket of $\mathcal{L}_{n,p}$.
\end{proof}
From the definition of $\eta$, one observes that for all $1\leq{r}\leq{n-1}$, $\eta$ operates on the elements of $\sfrac{\gamma_{r}\mathcal{L}_{n,p}}{\gamma_{r+1}\mathcal{L}_{n,p}}$ as the permutation: \[  \begin{pmatrix}
    1 & 2 & \cdots & n-r-1 & n-r \\
    n-r & n-r-1 & \cdots & 2 & 1
  \end{pmatrix}\]
Which means that, denoting by $M^{\eta}$ the matrix representing $\eta$, each diagonal block $M^{\eta}_{rr}$ is an anti-diagonal matrix with $1$ on the anti-diagonal.
\begin{corollary2}
Let $\eta\in{G_{n}(\mathbb{Q}_{p})}$ be the automorphism defined above, and let $G_{n}^{0}(\mathbb{Q}_{p}):=\{\varphi\in{G_{n}(\mathbb{Q}_{p})} : \mathrm{block}\,M_{11}\,\mathrm{is}\,\mathrm{diagonal}\}$ be the subgroup of all diagonal automorphisms of $\mathcal{L}_{n,p}$. Then $G_{n}(\mathbb{Q}_{p})=G_{n}^{0}(\mathbb{Q}_{p})\coprod{G_{n}^{0}(\mathbb{Q}_{p})\eta}$.
\end{corollary2}
\begin{remark2}
One checks that $\sfrac{G_{n}}{G_{n}^{0}}=\{G_{n}^{0}(\mathbb{Q}_{p}),G_{n}^{0}(\mathbb{Q}_{p})\eta\}$
\end{remark2}
Replacing $\varphi$ by $\varphi\circ\eta$ if necessary, we may assume without loss of generality that $M_{11}$ is diagonal. Indeed, let $G_{n}^{0}(\mathbb{Q}_{p})\leq{G_{n}(\mathbb{Q}_{p})}$ be the subgroup of automorphisms with diagonal block $M_{11}$, then\\ $G_{n}(\mathbb{Q}_{p})=G_{n}^{0}(\mathbb{Q}_{p})\coprod{G_{n}(\mathbb{Q}_{p})}\eta$, and as in \cite[Proposition 2.1]{DuSautoyLubotzky} we may replace the domain of integration in \eqref{eq:p-adic.integral} by $G_{n}^{0}(\mathbb{Q}_{p})\cap{G_{n}^{+}(\mathbb{Q}_{p})}$ after a suitable renormalization of the Haar measure. We proceed to determine $G_{n}^{0}(\mathbb{Q}_{p})$.
We check, for any $\lambda_{1},\lambda_{2},\dots,\lambda_{n-1}\in\mathbb{Q}_{p}^{\ast}$, that the diagonal matrix \[h=\mathrm{diag}(\lambda_{1},\lambda_{2},\dots,\lambda_{n-1},\lambda_{1}\lambda_{2},\lambda_{2}\lambda_{3}\dots,\lambda_{n-2}\lambda_{n-1},\dots,\lambda_{1}\lambda_{2}\cdots\lambda_{n-2}\lambda_{n-1})\]
represents an automorphism of $\mathcal{L}_{n,p}$. Thus every $g\in{G_{n}^{0}(\mathbb{Q}_{p})}$ has a unique decomposition $g=uh$, where $h$ is of the above form and $u$ has $1$'s on the diagonal. It is easy to see that $\det{h}=\prod_{i=1}^{n-1}\lambda_i^{i(n-i)}$ by induction on $n$. Since $\det{u}=1$, it follows that $|\det{g}|_{p}^{s}=|\det{h}|_{p}^{s}$.

The collection $H(\mathbb{Q}_{p})$ of diagonal matrices $h$ as above is the reductive part of $G_{n}^{0}(\mathbb{Q}_{p})$. The collection $N(\mathbb{Q}_{p})$ of matrices $u$ as above is the unipotent radical of $G_{n}^{0}(\mathbb{Q}_{p})$. We aim to determine the structure of the unipotent radical $N(\mathbb{Q}_p)$ by decomposing it into an iterative semidirect product of abelian subgroups.
For all $2\leq{r}\leq{n-1}$ we denote by $N_{r}\leq{N(\mathbb{Q}_{p})}$ the subgroup of all automorphisms of $\mathcal{L}_{n,p}$, such that\\ $M_{11}=I_{n}$ and $M_{12}=M_{13}=\cdots=M_{1,r-1}=0$. In other words, $N_{r}$ is the kernel of the natural map $G_{n}^{0}(\mathbb{Q}_{p})\rightarrow{Aut_{\mathbb{Q}_{p}}(\sfrac{\mathcal{L}_{n,p}}{\gamma_{r}\mathcal{L}_{n,p}})}$. We can describe $N_{n-1}$ explicitly as the following set of block matrices \[
N_{n-1}=\left\{\begin{pmatrix}
I_{n-1} & 0 & \cdots & 0 & M_{1,n-1}\\
0 & I_{n-2} & \cdots & 0 & 0\\
\vdots & \vdots & \ddots & \vdots & \vdots\\
0 & 0 & \cdots & I_{2} & 0\\
0 & 0 & \cdots & 0 & 1\\
\end{pmatrix}\right\}
\]
where $M_{1,n-1}$ is an arbitrary $(n-1)\times{1}$ matrix with entries in $\mathbb{Q}_{p}$ and the $0$ blocks are zero matrices of suitable size. The map $\varphi\mapsto{M_{1,n-1}}$ for all $\varphi\in{N_{n-1}}$ gives an isomorphism $N_{n-1}\cong\mathbb{Q}_{p}^{n-1}$.







\begin{proposition2}
\label{block.1r.structure}
Let $\varphi_{r}\in{N(\mathbb{Q}_{p})}$ be a unipotent automorphism of $\mathcal{L}_{n,p}$ such that the matrix upper blocks $M_{1k}$, for all $2\leq{k}\leq{r-1}$, are zero matrices. Consider the $(n-1)\times{(n-r)}$ matrix $M_{1r}=(a_{ij})$. Then,
\begin{enumerate}
    \item Let $2\leq{r}<{n-2}$. If $a_{ij}\neq{0}$, then either $i=j$ or $i=j+r-1$, and we have the relation $a_{i+r,i+1}=-a_{ii}$.
    \item Let $r=n-2$. If $a_{ij}\neq{0}$, then either $i=j$ or $i=j+r-1$ or $(i,j)\in\{(1,2),(n-1,1)\}$, with the same relation as above.
\end{enumerate}
\end{proposition2}
\begin{proof}
From the relation $[\varphi_{r}(e_{k,k+1}),\varphi_{r}(e_{l,l+1})]=0$ where $l>k+1$, we deduce that $a_{ij}\neq{0}$ only if either $i=j$ or $i=j+r-1$ or\\ $(i,j)\in\{(r+1,1),(r+2,1),(n-r-2,n-r),(n-r-1,n-r)\}$. If $r<n-2$ then it follows from the conditions
\begin{align*}
[\varphi_{r}(e_{n-r-2,n-r-1}),\varphi_{r}(e_{n-r-2,n-r})]=0\\
[\varphi_{r}(e_{n-r-1,n-r}),\varphi_{r}(e_{n-r-2,n-r})]=0\\
[\varphi_{r}(e_{r+1,r+2}),\varphi_{r}(e_{r+1,r+3})]=0\\
[\varphi_{r}(e_{r+2,r+3}),\varphi_{r}(e_{r+1,r+3})]=0\\
\end{align*}
that the four exceptional cases cannot occur. When $r=n-2$, we have that $(n-r-2,n-r)=(0,2)$ and $(r+2,1)=(n,1)$ so these cases do not exist, but so are the four conditions above, which means that the two remaining cases, $(r+1,1)=(n-1,1)$ and $(n-r-1,n-r)=(1,2)$, do not necessarily vanish.
\end{proof}
\begin{proposition2}
Denote by $N_{r}:=\{\varphi_{r} : 2\leq{r}\leq{n-2}\}\subset{N(\mathbb{Q}_{p})}$ the set of all automorphisms of the form described in \ref{block.1r.structure}, then $N_{r}\leq{N(\mathbb{Q}_{p})}$. Note that $N_2=N(\mathbb{Q}_{p})$.
\end{proposition2}
\begin{proposition2}
\label{phi.r.k}
Let $2\leq{r}\leq{n-2}$, and let $0\leq{k}\leq{n-r}$, and let $a\in\mathbb{Q}_{p}$. We extend our notation of basis elements to include $e_{01}=e_{n,n+1}=0$.
\begin{enumerate}
\item There is an automorphism $\varphi_{r,k}(a)\in{N(\mathbb{Q}_{p})}$ determined by \[
    \varphi_{r,k}(a)(e_{i,i+1}):=\begin{cases}
        e_{k,k+1}+a{e_{k,k+r}} & : i=k\\
        e_{k+r,k+r+1}-a{e_{k+1,k+r+1}} & : i=k+r\\
        e_{i,i+1} & : i\notin\{k,k+r\}
    \end{cases}
\]
\item Suppose that $r=n-2$, let $(k,l)\in\{(1,2),(n-1,1)\}$, and let $a\in\mathbb{Q}_{p}$. There is an automorphism $\varphi_{n-2,k,l}(a)\in{G_{n}^{0}(\mathbb{Q}_{p})}$ determined by \[
    \varphi_{n-2,k,l}(a)(e_{i,i+1}):=\begin{cases}
        e_{k,k+1}+a{e_{l,l+r}} & : i=k\\
        e_{i,i+1} & : i\neq{k}
    \end{cases}
\]
    We denote $\varphi'_{n-2}(a):=\varphi_{n-2,1,2}(a)$ and $\varphi''_{n-2}(a):=\varphi_{n-2,n-1,1}(a)$.
\end{enumerate}
\end{proposition2}
\begin{proof}
We need to verify that for all $1\leq{i<j}\leq{n}$ and $1\leq{l<m}\leq{n}$ we have the following relations \[
    [\varphi_{r,k}(a)(e_{ij}),\varphi_{r,k}(a)(e_{lm})]=\begin{cases}
    \varphi_{r,k}(a)(e_{im}) & : j=l\\
        -\varphi_{r,k}(a)(e_{lj}) & : i=m\\
        0 & : \mathrm{otherwise}
    \end{cases}
\]
We can verify explicitly for $n=4$ that these relations are true. Alternatively, Berman did this in \cite[\S{3.3.7}]{BermanThesis}. For $n>4$, let $m=n$, then \[[\varphi_{r,k}(a)(e_{ij}),\varphi_{r,k}(a)(e_{lm})]=[\varphi_{r,k}(a)(e_{ij}),\varphi_{r,k}(a)(e_{ln})].\]
If $i>1$, then we consider the inclusion $\iota:\mathcal{L}_{n-1,p}\hookrightarrow\mathcal{L}_{n,p}$, mapping each $e_{i,i+1}\in\mathcal{L}_{n-1,p}$ to $e_{i+1,i+2}\in\mathcal{L}_{n,p}$ for all $1\leq{i}\leq{n-2}$. By the assumption on $\mathcal{L}_{n-1,p}$, we have that \[
(\iota\circ\iota^{-1})([\varphi_{r,k}(a)(e_{ij}),\varphi_{r,k}(a)(e_{ln})])=\iota([\iota^{-1}(\varphi_{r,k}(a)(e_{ij})),\iota^{-1}(\varphi_{r,k}(a)(e_{ln}))])=\]\[=\iota([\varphi_{r,k}(a)(e_{i-1,j-1}),\varphi_{r,k}(a)(e_{l-1,n-1})])=\]\[=\begin{cases}
\iota(\varphi_{r,k}(a)(e_{i-1,n-1}))=\varphi_{r,k}(a)(e_{in}) & : j=l\\
        0 & : j\neq{l}
    \end{cases}
\]
If $i=1$, then \[[\varphi_{r,k}(a)(e_{ij}),\varphi_{r,k}(a)(e_{ln})]=[\varphi_{r,k}(a)(e_{1j}),\varphi_{r,k}(a)(e_{ln})]=\]\[=[\varphi_{r,k}(a)(e_{1j}),[\varphi_{r,k}(a)(e_{l,n-1}),\varphi_{r,k}(a)(e_{n-1,n})]].\]
By the Jacobi identity, we have that \[[\varphi_{r,k}(a)(e_{1j}),[\varphi_{r,k}(a)(e_{l,n-1}),\varphi_{r,k}(a)(e_{n-1,n})]]=\]\[=-[\varphi_{r,k}(a)(e_{n-1,n}),[\varphi_{r,k}(a)(e_{1j}),\varphi_{r,k}(a)(e_{l,n-1})]].\]
Now we use the inclusion $\iota':\mathcal{L}_{n-1,p}\hookrightarrow\mathcal{L}_{n,p}$, where $\iota'(e_{i,i+1})=e_{i,i+1}$ for all $1\leq{i}\leq{n-1}$, to obtain, same as above, that \[-[\varphi_{r,k}(a)(e_{n-1,n}),[\varphi_{r,k}(a)(e_{1j}),\varphi_{r,k}(a)(e_{l,n-1})]]=-[\varphi_{r,k}(a)(e_{n-1,n}),\varphi_{r,k}(a)(e_{1,n-1})].\]
To continue, we need to prove the following auxiliary proposition:
\begin{proposition2}
\label{phi.r.k.general.element}
\[\varphi_{r,k}(a)(e_{k+1-h,k+1})=e_{k+1-h,k+1}+ae_{k+1-h,k+r} : h>0\]
\[\varphi_{r,k}(a)(e_{k+r,k+r+h})=e_{k+r,k+r+h}-ae_{k+1,k+r+h} : h>0\]
\[\varphi_{r,k}(a)(e_{ij})=e_{ij} : i\neq{k+r}\land{j\neq{k+1}}\] 
\end{proposition2}
\begin{proof}
For $h=1$, $\varphi_{r,k}(a)(e_{k,k+1})=e_{k,k+1}+ae_{k,k+r}$. For $h'=h>1$, $\varphi_{r,k}(a)(e_{k+1-h',k+1})=[\varphi_{r,k}(a)(e_{k-h,k-h+1}),\varphi_{r,k}(a)(e_{k-h+1,k+1})]$. By the assumption, we have that $[\varphi_{r,k}(a)(e_{k-h,k-h+1}),\varphi_{r,k}(a)(e_{k-h+1,k+1})]=$\[=[\varphi_{r,k}(a)(e_{k-h,k-h+1}),e_{k+1-h,k+1}+ae_{k+1-h,k+r}].\]
But for all $h>0$, we have that $k-h\neq{k}$ and $k-h+1\neq{k+1}$, and hence \[[\varphi_{r,k}(a)(e_{k-h,k-h+1}),e_{k+1-h,k+1}+ae_{k+1-h,k+r}]=\]\[=[e_{k-h,k-h+1},e_{k+1-h,k+1}+ae_{k+1-h,k+r}=e_{k-h,k+1}+ae_{k-h,k+r}=\]\[=e_{k+1-h',k+1}+ae_{k+1-h',k+r}.\]
We prove the two other cases in the same way.
\end{proof}
By \ref{phi.r.k.general.element} we have that 
\[\varphi_{r,k}(a)(e_{1,n-1})=\begin{cases}
        e_{1,n-1}+ae_{1,n} & : r=2\land{k=n-2}\\
        e_{1,n-1} & : \mathrm{otherwise}
    \end{cases}
\]
while $k+r\neq{1}$ for all $r,k$. Thus, $-[\varphi_{2,n-2}(a)(e_{n-1,n}),\varphi_{2,n-2}(a)(e_{1,n-1})]=-[\varphi_{2,n-2}(a)(e_{n-1,n}),e_{1,n-1}+ae_{1,n}]=[e_{n-1,n},e_{1,n-1}+ae_{1,n}]=e_{1n}$. 

For $(r,k)\notin(2,n-2)$, if $k+r=n-1$ then $-[\varphi_{r,k}(a)(e_{n-1,n}),\varphi_{r,k}(a)(e_{1,n-1})]=-[e_{n-1,n}-ae_{n-r,n},e_{1,n-1}]=e_{1n}$, otherwise $-[\varphi_{r,k}(a)(e_{n-1,n}),\varphi_{r,k}(a)(e_{1,n-1})]=-[e_{n-1,n},e_{1,n-1}]=e_{1n}$
\end{proof}
Fix the two parameters $2\leq{r}\leq{n-2}$ and $0\leq{k}\leq{n-r}$, and denote by $N_{r,k}:=\{\varphi_{r,k}(a) : a\in\mathbb{Q}_{p}\}\subset{N(\mathbb{Q}_{p})}$ the set of all automorphisms of this form. Also denote $N'_{n-2}:=\{\varphi'_{n-2}(a) : a\in\mathbb{Q}_{p}\}$ and $N''_{n-2}:=\{\varphi''_{n-2}(a) : a\in\mathbb{Q}_{p}\}.$
\begin{proposition2}
Let $N_{r,k}$, $N'_{n-2}$ and $N''_{n-2}$ be the subsets defined above, then
\begin{enumerate}
    \item $N_{r,k},N'_{n-2},N''_{n-2}\leq{N(\mathbb{Q}_{p})}.$
    \item $N_{r,k},N'_{n-2},N''_{n-2}\cong{\mathbb{Q}_{p}}.$
\end{enumerate}
\end{proposition2}
\begin{proof}
A simple check shows that these subsets are subgroups of $N(\mathbb{Q}_p)$. Define $\tau_{r,k}:\mathbb{Q}_{p}\rightarrow{N_{r,k}}$. For every $a,b\in\mathbb{Q}_{p}$, it is easy to see that the image of the sum, $\tau_{r,k}(a+b)=\tau_{r,k}(a)\cdot\tau_{r,k}(b)$, is the product of the images of $a$ and $b$, and that $\tau_{r,k}^{-1}(I)=\{0\}$.
\end{proof}
The following proposition follows from a simple computation.
\begin{proposition2}
\label{prop:psi.automorphism}
Consider $\varphi_{r}\in{N_{r}}$.
\begin{enumerate}
    \item 
If $r<n-2$, denote by $\psi_{r}$ the automorphism \[\psi_{r}:=\varphi_{r}\circ\varphi_{r,n-r}(-a_{n-r,n-r})\circ\cdots\circ\varphi_{r,1}(-a_{11})\circ\varphi_{r,0}(-a_{r+1,1}).\]
Then $\psi_{r}\in{N_{r+1}}$.
    \item 
If $r=n-2$, denote by $\psi_{n-2}$ the automorphism \[\psi_{n-2}:=\varphi_{r}\circ\varphi'_{n-2}(-a_{12})\circ\varphi''_{n-2}(-a_{n-1,1})\circ\]\[\circ\varphi_{n-2,2}(-a_{n-2,2})\circ\varphi_{n-2,1}(-a_{n-2,1})\circ\varphi_{n-2,0}(-a_{n-2,0}).\]
Then $\psi_{n-2}\in{N_{n-1}}$.
\end{enumerate}
\end{proposition2}
\begin{proof}
By the definition, $\varphi_{r}$ has $1$ on the main diagonal and all the upper blocks $M_{1k}$, for $2\leq{k}\leq{r-1}$ are zero matrices. One checks that the composition of $\varphi_{r}$ and the chain of compositions $\prod_{k=1}^{n-r}\varphi_{r,k}(-a_{kk})\circ\varphi_{r,0}(-a_{r+1,1})$ yields also a matrix with $1$ on the main diagonal whose upper blocks $M_{1k}$, for all $2\leq{k}\leq{r}$, are zero matrices, thus $\psi_{r}\in{N_{r+1}}$. Same applies for the case $r=n-2$, considering the specific structure of $M_{1,n-2}$, as described in the second part of \ref{block.1r.structure}.
\end{proof}
\begin{corollary2}
\label{cor:Nr.decomposition}
We have the following decompositions:
\begin{enumerate}
    \item 
For all $2\leq{r}<{n-2}$, we have \[N_{r}=N_{r+1}\rtimes(N_{r,0}\rtimes(\cdots(N_{r,n-r-1}\rtimes{N_{r,n-r}})\cdots)).\]
\item For $r=n-2$, we have 
\[N_{n-2}=N_{n-1}\rtimes({N_{n-2,0}}\rtimes(N_{n-2,1}\rtimes(N_{n-2,2}\rtimes(N''_{n-2}\rtimes{N'_{n-2}})))).\]
\end{enumerate}
\end{corollary2}
\begin{proof}
This is immediate from Proposition \ref{prop:psi.automorphism}, since we have that \[\varphi_{r}=\psi_{r}\circ\varphi_{r,0}(-a_{r+1,1})\circ\varphi_{r,1}(-a_{11})\circ\cdots\circ\varphi_{r,n-r}(-a_{n-r,n-r}).\]
\end{proof}
Corollary \ref{cor:Nr.decomposition} provides a recursive decomposition of the unipotent radical $N(\mathbb{Q}_{p})$ as an iterated semidirect product of $N_{n-1}$ and subgroups isomorphic to $\mathbb{Q}_{p}$.

As we saw earlier, the calculation of $\zeta_{L_{n,p}}^{\wedge}(s)$ requires understanding $G_{n}(\mathbb{Z}_p)$ and $G_{n}^{+}(\mathbb{Q}_p)$ first. As $G_{n}(\mathbb{Z}_{p})$ is a group, its structure is easily deduced from the above.
\begin{proposition2}
\label{prop:G.n.Zp.decomposition}
For all $n\geq{4}$ the group $G_{n}^{0}(\mathbb{Z}_{p})$ has the decomposition $G_{n}^{0}(\mathbb{Z}_{p})=N(\mathbb{Z}_{p})\rtimes{H(\mathbb{Z}_{p})}$, where \[N(\mathbb{Z}_{p}):=M_{\binom{n}{2}}(\mathbb{Z}_{p})\cap{N(\mathbb{Q}_{p})},\]
\[H(\mathbb{Z}_{p}):=\{\mathrm{diag}(\lambda_{1},\lambda_{2},\dots,) : \lambda_1,\dots,\lambda_{n-1}\in\mathbb{Z}_{p}^{\ast}\}.\]
Moreover, $N(\mathbb{Z}_{p})$ itself has the decomposition: \[N(\mathbb{Z}_{p})=\Tilde{N}_{2}(\mathbb{Z}_{p})=
\Tilde{N}_{n-1}\rtimes({\Tilde{N}_{n-2,0}}\rtimes(\Tilde{N}_{n-2,1}\rtimes(\Tilde{N}_{n-2,2}\rtimes(\Tilde{N}''_{n-2}\rtimes{\Tilde{N}'_{n-2}}))))\rtimes\cdots\]\[\cdots\rtimes{(\Tilde{N}_{2,0}\rtimes(\cdots(\Tilde{N}_{2,n-3}\rtimes{\Tilde{N}_{2,n-2}})\cdots))}
,\]
where $\Tilde{N}_{r}=N_{r}\cap{N(\mathbb{Z}_{p})}$ and $\Tilde{N}_{r,k}=\{\varphi_{r,k}(a) : a\in\mathbb{Z}_{p}\}$.
\end{proposition2}
By contrast, describing the structure of the monoid $G_{n}^{+}(\mathbb{Q}_p)$ is expected to be a substantial challenge.

By applying Fubini's theorem for semidirect products of topological groups \cite[Proposition 28]{Nachbin}, we have that \[\zeta_{L_{n,p}}^{\wedge}(s)=\displaystyle\int_{G_{n}^{+}(\mathbb{Q}_p)}|\det{\varphi}|_p^sd\mu_{G_{n}(\mathbb{Z}_p)\varphi}=\displaystyle\int_{H^+(\mathbb{Q}_p)}\left(\displaystyle\int_{N_{h}^+}|\det{uh}|_p^sd\mu_{N(\mathbb{Q}_p)}\right)d\mu_{H(\mathbb{Q}_p)},\]
where \[H^+(\mathbb{Q}_p):=\{\mathrm{diag}(\lambda_{1},\dots,\lambda_{n-1},\lambda_{1}\lambda_{2},\dots,\lambda_{1}\lambda_{2}\cdots\lambda_{n-2}\lambda_{n-1}) : \lambda_{i}\in\mathbb{Z}_{p}\setminus\{0\}\},\]
that is, $H^+(\mathbb{Q}_p)$ consists of all $h\in{H(\mathbb{Q}_{p})}$ that appear in the decomposition $\varphi=uh$ for some $\varphi\in{G_{n}^{+}(\mathbb{Q}_{p})}$, and, for a given $h\in{H^{+}(\mathbb{Q}_{p})}$, we set $N_{h}^{+}:=\{u\in{N(\mathbb{Q}_{p}) : uh\in{G_{n}^{+}(\mathbb{Q}_{p})}}\}$. The integrand is constant on $N_{h}^{+}$, so computing the inner integral amounts to finding the measure of $N_{h}^+$, which is complicated, but using the decomposition from Corollary \ref{cor:Nr.decomposition}, we can simplify $N_{h}^{+}$ at the price of replacing a single integral by multiple integrals.

Let $\mathcal{N}_{1},\mathcal{N}_{2},\dots,\mathcal{N}_{m}$, where $m=\binom{n}{2}$, be an enumeration of the subgroups
\[N_{2,n-2},N_{2,n-3},\dots,N_{2,0},N_{3,n-3},\dots,N_{3,0},\dots\]\[\dots,N_{n-2,2},N_{n-2,1},N_{n-2,0},N'_{n-2},N''_{n-2},N_{n-1}.\]
Every $\varphi\in{G_{n}^{0}(\mathbb{Q}_{p})}$ can be written uniquely as $\varphi=u_{m}\cdots{u_{1}h}$, where $u_{i}\in{\mathcal{N}_{i}}$. Thus, by Fubini \[
\zeta_{L_{n,p}}^{\wedge}(s)=\displaystyle\int_{H^{+}}\displaystyle\int_{\mathcal{N}_{1}^{+}(h)}\displaystyle\int_{\mathcal{N}_{2}^{+}(h,u_{1})}\cdots\displaystyle\int_{\mathcal{N}_{m}^{+}(h,u_{1},\dots,u_{m-1})}|\det{h}|_{p}^{s}d\mu_{H}d\mu_{\mathcal{N}_{1}}\cdots{d\mu_{\mathcal{N}_{m}}},\]
where each $\mu_{\mathcal{N}_{i}}$ is Haar measure on $\mathcal{N}_{i}(\mathbb{Q}_{p})$ normalized so that\\ $\mu_{\mathcal{N}_{i}}(\mathcal{N}_{i}(\mathbb{Z}_{p}))=1$, and \[\mathcal{N}_{i}^{+}(h,u_{1},\dots,u_{i-1}):=\{u_{i}\in\mathcal{N}_{i} : \exists{u_{i+1},\dots,u_{m}}\,\mathrm{such}\,\mathrm{that}\,u_{m}\cdots{u_{1}}h\in{G_{n}^{+}(\mathbb{Q}_{p})}\}.\]
\end{document}
