\documentclass{article}
\usepackage{graphicx} % Required for inserting images
\usepackage{amsmath}
\usepackage{amsfonts}
\title{cases}
\author{haiml76 }
\date{July 2025}

\begin{document}

\maketitle
Denote $p^{\min}:=p^{\min\{0,v_2+v_{11}\}}$

Denote $\rho:=(1-p^{-1})$

Denote $f(p,t)$ the $p$ and $t$ product $p^{7v_1+10v_2+11v_3+7v_4+\min\{v_1,v_4\}}t^{4v_1+6v_2+6v_3+4v_4}$
\section{Case 1}
$v_3>v_1\geq{v_4}>v_2\geq{0}$

$\Rightarrow{v_{11}}\geq{-v_2-v_1}$

$\Rightarrow\alpha:=\min\{v_2,v_2+v_{11}+v_1\}=     \begin{cases}
       v_2, & v_{11}\geq{-v_1}\\
       v_2-1,v_2-2,\dots, & v_{11}<{-v_1}\\
     \end{cases}$

    $\Rightarrow{f(p,t)=p^{7v_1+10v_2+11v_3+7v_4+v_4}t^{4v_1+6v_2+6v_3+4v_4}=p^{7v_1+10v_2+11v_3+8v_4}t^{4v_1+6v_2+6v_3+4v_4}}$
\begin{enumerate}
    \item 
For $v_{11}\geq{-v_2}$, we have $p^{\min}(1+\alpha\rho)\mu(a_{11})=p^{v_2}(1+v_2\rho)$.
\item
For $-v_1\leq{v_{11}}\leq{-v_2-1}$, we have $p^{\min}(1+\alpha\rho)\mu(a_{11})=\sum_{-v_1}^{-v_2-1}p^{v_2}\rho(1+v_2\rho)=p^{v_2}(v_1-v_2)\rho(1+v_2\rho)=p^{v_2}(v_1-v_2)\rho+p^{v_2}v_2(v_1-v_2)\rho^2$.
\item
For $-v_2-v_1\leq{v_{11}}\leq{-v_1-1}$, we have $p^{\min}(1+\alpha\rho)\mu(a_{11})=\sum_{-v_2-v_1}^{-v_1-1}p^{v_2}\rho(1+\alpha\rho)=\sum_{i=1}^{v_2}p^{v_2}\rho(1+(v_2-i)\rho)=p^{v_2}v_2\rho+p^{v_2}v_2^2\rho^2-p^{v_2}\binom{v_2+1}{2}\rho^2.$
\end{enumerate}
So we have $\sum_{v_{11}\geq{-v_2-v_1}}=p^{v_2}(1+v_2\rho+(v_1-v_2)\rho+v_2(v_1-v_2)\rho^2+v_2\rho+v_2^2\rho^2-\frac{(v_2+1)v_2}{2}\rho^2)=p^{v_2}(1+v_1\rho+v_2v_1\rho^2+v_2\rho-\frac{v_2^2}{2}\rho^2-\frac{v_2}{2}\rho^2).$
We compute the differences between $v_1,v_2,v_3,v_4$,

$v_3\overset{d}{>}v_1\overset{c}{\geq}{v_4}\overset{b}>v_2\overset{a}{\geq}{0}$

Thus, we substitute $v_1\rightarrow{a+b+c}$, $v_2\rightarrow{a}$, $v_3\rightarrow{a+b+c+d}$, $v_4\rightarrow{a+b}$, and compute series with the new variables as indices, where $a,c\geq{0}$ and $b,d\geq{1}$.

\section{Case 2}
$v_1\geq{v_3}\geq{0}$

$v_1\geq{v_4}>v_2\geq{0}$

$\Rightarrow{v_{11}}\geq{-v_2-v_3}$

$\Rightarrow\alpha:=\min\{v_2,v_2+v_{11}+v_1\}=\begin{cases}
       v_2, & v_{11}\geq{-v_1}\\
       v_2-1,v_2-2,\dots, & v_{11}<{-v_1}\\
     \end{cases}$

     $\Rightarrow{f(p,t)=p^{7v_1+10v_2+11v_3+7v_4+v_4}t^{4v_1+6v_2+6v_3+4v_4}=p^{7v_1+10v_2+11v_3+8v_4}t^{4v_1+6v_2+6v_3+4v_4}}$

We have two sub cases.
\subsection{Sub case 2.1}
$-v_2-v_3\geq{-v_1}\Rightarrow{v_1\geq{v_2+v_3}}$

Here there is no phase transition, because the phase transition occurs at $-v_1-1<{-v_2-v_3}\leq{v_{11}}$
\begin{enumerate}
    \item 
For $v_{11}\geq{-v_2}$, we have $p^{\min}(1+\alpha\rho)\mu(a_{11})=p^{v_2}(1+v_2\rho)$.
\item 
For $-v_2-v_3\leq{v_{11}}\leq{-v_2-1}$, we have $p^{\min}(1+\alpha\rho)\mu(a_{11})=\sum_{-v_2-v_3}^{-v_2-1}p^{v_2}\rho(1+v_2\rho)=p^{v_2}v_3\rho(1+v_2\rho)=p^{v_2}v_3\rho+p^{v_2}v_3v_2\rho^2$.
\end{enumerate}
So we have $\sum_{v_{11}\geq{-v_2-v_3}}=p^{v_2}(1+v_2\rho+v_3\rho+v_2v_3\rho^2).$

We compute the differences between $v_1,v_2,v_3,v_4$, we have several arrangements,
\begin{enumerate}
    \item 
$v_1\overset{d}{\geq}{v_2+v_3}\overset{a}{\geq}v_3\overset{c}{\geq}{v_4}\overset{b}>v_2\overset{a}{\geq}{0}$

Thus, we substitute $v_1\rightarrow{2a+b+c+d}$, $v_2\rightarrow{a}$, $v_3\rightarrow{a+b+c}$, $v_4\rightarrow{a+b}$, and compute series with the new variables as indices, where $a,c,d\geq{0}$ and $b\geq{1}$.
\item 
$v_1\overset{d}{\geq}{v_2+v_3}\overset{c}{\geq}v_4\overset{b}{>}{v_3}\overset{a}{>}v_2\overset{e}{\geq}{0}$

But $v_2+v_3-c-b=v_3\Rightarrow{v_2=v_2+v_3-v_3=b+c}$

Thus, we substitute $v_1\rightarrow{a+2b+2c+d}$, $v_2\rightarrow{b+c}$, $v_3\rightarrow{a+b+c}$, $v_4\rightarrow{a+2b+c}$, and compute series with the new variables as indices, where $c,d\geq{0}$ and $a,b\geq{1}$.

\item 
$v_1\overset{d}{\geq}{v_2+v_3}\overset{c}{\geq}v_4\overset{b}{>}{v_2}\overset{a}{\geq}v_3\overset{e}{\geq}{0}$

But $v_2+v_3-c-b=v_2\Rightarrow{v_3=v_2+v_3-v_2=b+c}$

Thus, we substitute $v_1\rightarrow{a+2b+2c+d}$, $v_2\rightarrow{a+b+c}$, $v_3\rightarrow{b+c}$, $v_4\rightarrow{a+2b+c}$, and compute series with the new variables as indices, where $a,c,d\geq{0}$ and $b\geq{1}$.

\item 
$v_1\overset{d}{\geq}{v_4}\overset{c}{>}v_2+v_3\overset{a}{\geq}{v_2}\overset{b}{\geq}v_3\overset{a}{\geq}{0}$

Thus, we substitute $v_1\rightarrow{2a+b+c+d}$, $v_2\rightarrow{a+b}$, $v_3\rightarrow{a}$, $v_4\rightarrow{2a+b+c}$, and compute series with the new variables as indices, where $a,b,d\geq{0}$ and $c\geq{1}.$

\item 
$v_1\overset{d}{\geq}{v_4}\overset{c}{>}v_2+v_3\overset{a}{\geq}{v_3}\overset{b}{>}v_2\overset{a}{\geq}{0}$

Thus, we substitute $v_1\rightarrow{2a+b+c+d}$, $v_2\rightarrow{a}$, $v_3\rightarrow{a+b}$, $v_4\rightarrow{2a+b+c}$, and compute series with the new variables as indices, where $a,d\geq{0}$ and $b,c\geq{1}.$
\end{enumerate}
\subsection{Sub case 2.2}
$-v_2-v_3<{-v_1}\Rightarrow{v_1<{v_2+v_3}}$
\begin{enumerate}
    \item 
For $v_{11}\geq{-v_2}$, we have $p^{\min}(1+\alpha\rho)\mu(a_{11})=p^{v_2}(1+v_2\rho)$.
\item 
For $-v_1\leq{v_{11}}\leq{-v_2-1}$, we have $p^{\min}(1+\alpha\rho)\mu(a_{11})=\sum_{-v_1}^{-v_2-1}p^{v_2}\rho(1+v_2\rho)=p^{v_2}(v_1-v_2)\rho(1+v_2\rho)=p^{v_2}(v_1-v_2)\rho+p^{v_2}(v_1-v_2)v_2\rho^2$.
\item 
For $-v_2-v_3\leq{v_{11}}\leq{-v_1-1}$, we have $p^{\min}(1+\alpha\rho)\mu(a_{11})=\sum_{-v_2-v_3}^{-v_1-1}p^{v_2}\rho(1+\alpha\rho)=\sum_{i=1}^{v_2+v_3-v_1}p^{v_2}\rho(1+(v_2-i)\rho)=p^{v_2}(v_2+v_3-v_1)\rho+p^{v_2}(v_2+v_3-v_1)v_2\rho^2-p^{v_2}\binom{v_2+v_3-v_1+1}{2}\rho^2$.
\end{enumerate}
So we have $\sum_{v_{11}\geq{-v_2-v_3}}=p^{v_2}(1+v_2\rho+(v_1-v_2)\rho+(v_1-v_2)v_2\rho^2+(v_2+v_3-v_1)\rho+(v_2+v_3-v_1)v_2\rho^2-\frac{(v_2+v_3-v_1+1)(v_2+v_3-v_1)}{2}\rho^2)=p^{v_2}(1+v_2\rho+v_3\rho-\frac{v_2^2}{2}\rho^2+\frac{v_2v_1}{2}\rho^2-\frac{v_3^2}{2}\rho^2+\frac{v_3v_1}{2}\rho^2+\frac{v_1v_2}{2}\rho^2+\frac{v_1v_3}{2}\rho^2-\frac{v_1^2}{2}\rho^2-\frac{v_2}{2}\rho^2-\frac{v_3}{2}\rho^2+\frac{v_1}{2}\rho^2)=p^{v_2}(1+v_2\rho+v_3\rho-\frac{v_2^2}{2}\rho^2+v_2v_1\rho^2-\frac{v_3^2}{2}\rho^2+v_3v_1\rho^2-\frac{v_1^2}{2}\rho^2-\frac{v_2}{2}\rho^2-\frac{v_3}{2}\rho^2+\frac{v_1}{2}\rho^2).$
We compute the differences between $v_1,v_2,v_3,v_4$, we have several arrangements,
\begin{enumerate}
    \item 
$v_2+v_3\overset{d}{>}v_1\overset{c}{\geq}v_3\overset{b}{\geq}{v_4}\overset{a}>v_2\overset{e}{\geq}{0}$

But $v_2+v_3-d-c=v_3\Rightarrow{v_2=c+d}$

Thus, we substitute 
$v_1\rightarrow{a+b+2c+d}$, 
$v_2\rightarrow{c+d}$, 
$v_3\rightarrow{a+b+c+d}$, 
$v_4\rightarrow{a+c+d}$, and compute series with the new variables as indices, where $b,c\geq{0}$ and $a,d\geq{1}$.

\item 
$v_2+v_3\overset{d}{>}v_1\overset{c}{\geq}v_4\overset{b}{>}{v_3}\overset{a}>v_2\overset{e}{\geq}{0}$

But $v_2+v_3-d-c-b=v_3\Rightarrow{v_2=v_2+v_3-v_3=b+c+d}$

Thus, we substitute 
$v_1\rightarrow{a+2b+2c+d}$, 
$v_2\rightarrow{b+c+d}$, 
$v_3\rightarrow{a+b+c+d}$, 
$v_4\rightarrow{a+2b+c+d}$, and compute series with the new variables as indices, where $c\geq{0}$ and $a,b,d\geq{1}$.

\item 
$v_2+v_3\overset{d}{>}v_1\overset{c}{\geq}v_4\overset{b}{>}{v_2}\overset{a}{\geq}v_3\overset{e}{\geq}{0}$

But $v_2+v_3-d-c-b=v_2\Rightarrow{v_3=v_2+v_3-v_2=b+c+d}$

Thus, we substitute 
$v_1\rightarrow{a+2b+2c+d}$, 
$v_2\rightarrow{a+b+c+d}$, 
$v_3\rightarrow{b+c+d}$, 
$v_4\rightarrow{a+2b+c+d}$, and compute series with the new variables as indices, where $a,c\geq{0}$ and $b,d\geq{1}$.

\end{enumerate}

\section{Case 3}
$v_3>v_1\geq{0}$

$v_4>v_1\geq{0}$

$v_4>v_2\geq{0}$

$\Rightarrow{v_{11}}\geq{-v_2-v_1}$

$\Rightarrow\alpha:=\min\{v_2,v_2+v_{11}+v_4\}=\begin{cases}
       v_2, & v_{11}\geq{-v_4}\\
       v_2-1,v_2-2,\dots, & v_{11}<{-v_4}\\
     \end{cases}$

     $\Rightarrow{f(p,t)=p^{7v_1+10v_2+11v_3+7v_4+v_1}t^{4v_1+6v_2+6v_3+4v_4}=p^{8v_1+10v_2+11v_3+7v_4}t^{4v_1+6v_2+6v_3+4v_4}}$

We have two sub cases

\subsection{Sub case 3.1}
$-v_2-v_1>-v_4\Rightarrow{v_4>v_2+v_1}$

There is no phase transition here, since $v_{11}\geq{-v_2-v_1}>-v_4$
\begin{enumerate}
    \item 
For $v_{11}\geq{-v_2}$, we have $p^{\min}(1+\alpha\rho)\mu(a_{11})=p^{v_2}(1+v_2\rho)$.
\item 
For $-v_2-v_1\leq{v_{11}}\leq{-v_2-1}$, we have $p^{\min}(1+\alpha\rho)\mu(a_{11})=\sum_{-v_2-v_1}^{-v_2-1}p^{v_2}\rho(1+v_2\rho)=p^{v_2}v_1\rho+p^{v_2}v_1v_2\rho^2$.
\end{enumerate}
So we have $\sum_{v_{11}\geq{-v_2-v_1}}p^{\min}(1+\alpha\rho)\mu(a_{11})=p^{v_2}(1+v_2\rho+v_1\rho+v_1v_2\rho^2).$

We have several arrangements,

\begin{enumerate}
\item 
$v_4\overset{d}{>}v_1+v_2\overset{c}{\geq}v_3\overset{b}{>}{v_2}\overset{a}{>}v_1\overset{e}{\geq}{0}$

But $v_1+v_2-c-b=v_2\Rightarrow{v_1=v_1+v_2-v_2=b+c}$

Thus, we substitute 
$v_1\rightarrow{b+c}$, 
$v_2\rightarrow{a+b+c}$, 
$v_3\rightarrow{a+2b+c}$, 
$v_4\rightarrow{a+2b+2c+d}$, and compute series with the new variables as indices, where $c\geq{0}$ and $a,b,d\geq{1}$.
\item 
$v_4\overset{d}{>}v_1+v_2\overset{a}{\geq}v_2\overset{c}{\geq}{v_3}\overset{b}{>}v_1\overset{a}{\geq}{0}$

We substitute 
$v_1\rightarrow{a}$, 
$v_2\rightarrow{a+b+c}$, 
$v_3\rightarrow{a+b}$, 
$v_4\rightarrow{2a+b+c+d}$, and compute series with the new variables as indices, where $a,c\geq{0}$ and $b,d\geq{1}$.
\item 
$v_4\overset{d}{>}v_1+v_2\overset{c}{\geq}v_3\overset{b}{>}{v_1}\overset{a}{\geq}v_2\overset{e}{\geq}{0}$

But $v_1+v_2-c-b=v_1\Rightarrow{v_2=v_1+v_2-v_1=b+c}$

We substitute 
$v_1\rightarrow{a+b+c}$, 
$v_2\rightarrow{b+c}$, 
$v_3\rightarrow{a+2b+c}$, 
$v_4\rightarrow{a+2b+2c+d}$, and compute series with the new variables as indices, where $a,c\geq{0}$ and $b,d\geq{1}$.
\item 
$v_4\overset{d}{>}v_3\overset{c}{>}v_1+v_2\overset{a}{\geq}{v_1}\overset{b}{\geq}v_2\overset{a}{\geq}{0}$

We substitute 
$v_1\rightarrow{a+b}$, 
$v_2\rightarrow{a}$, 
$v_3\rightarrow{2a+b+c}$, 
$v_4\rightarrow{2a+b+c+d}$, and compute series with the new variables as indices, where $a,b\geq{0}$ and $c,d\geq{1}$.
\item 
$v_4\overset{d}{>}v_3\overset{c}{>}v_1+v_2\overset{a}{\geq}{v_2}\overset{b}{>}v_1\overset{a}{\geq}{0}$

We substitute 
$v_1\rightarrow{a}$, 
$v_2\rightarrow{a+b}$, 
$v_3\rightarrow{2a+b+c}$, 
$v_4\rightarrow{2a+b+c+d}$, and compute series with the new variables as indices, where $a\geq{0}$ and $b,c,d\geq{1}$.

\item 
$v_3\overset{d}{\geq}v_4\overset{c}{>}v_1+v_2\overset{a}{\geq}{v_2}\overset{b}{>}v_1\overset{a}{\geq}{0}$

We substitute 
$v_1\rightarrow{a}$, 
$v_2\rightarrow{a+b}$, 
$v_3\rightarrow{2a+b+c+d}$, 
$v_4\rightarrow{2a+b+c}$, and compute series with the new variables as indices, where $a,d\geq{0}$ and $b,c\geq{1}$.
\item 
$v_3\overset{d}{\geq}v_4\overset{c}{>}v_1+v_2\overset{a}{\geq}{v_1}\overset{b}{\geq}v_2\overset{a}{\geq}{0}$

We substitute 
$v_1\rightarrow{a+b}$, 
$v_2\rightarrow{a}$, 
$v_3\rightarrow{2a+b+c+d}$, 
$v_4\rightarrow{2a+b+c}$, and compute series with the new variables as indices, where $a,b,d\geq{0}$ and $c\geq{1}$.
\end{enumerate}
\subsection{Sub case 3.2}
$-v_4\geq{-v_2-v_1}\Rightarrow{v_2+v_1\geq{v_4}}$
\begin{enumerate}
    \item 
For $v_{11}\geq{-v_2}$, we have $p^{\min}(1+\alpha\rho)\mu(a_{11})=p^{v_2}(1+v_2\rho)$.
\item 
For $-v_4\leq{v_{11}}\leq{-v_2-1}$, we have $p^{\min}(1+\alpha\rho)\mu(a_{11})=\sum_{-v_4}^{-v_2-1}p^{v_2}\rho(1+v_2\rho)=p^{v_2}(v_4-v_2)\rho+p^{v_2}(v_4-v_2)v_2\rho^2$.
\item 
For $-v_2-v_1\leq{v_{11}}\leq{-v_4-1}$, we have $p^{\min}(1+\alpha\rho)\mu(a_{11})=\sum_{-v_2-v_1}^{-v_4-1}p^{v_2}\rho(1+v_2\rho)=\sum_{i=1}^{v_1+v_2-v_
4}p^{v_2}\rho(1+(v_2-i)\rho)=p^{v_2}(v_1+v_2-v_4)\rho+p^{v_2}(v_1+v_2-v_4)v_2\rho^2-p^{v_2}\binom{v_1+v_2-v_4+1}{2}\rho^2$.
\end{enumerate}
So we have $\sum_{v_{11}\geq{-v_2-v_1}}p^{\min}(1+\alpha\rho)\mu(a_{11})=p^{v_2}(1+v_2\rho+(v_4-v_2)\rho+(v_4-v_2)v_2\rho^2+(v_1+v_2-v_4)\rho+(v_1+v_2-v_4)v_2\rho^2-\frac{(v_1+v_2-v_4+1)(v_1+v_2-v_4)}{2}\rho^2)=p^{v_2}(1+v_1\rho+v_2\rho-\frac{v_1^2}{2}\rho^2+v_4v_1\rho^2-\frac{v_2^2}{2}\rho^2+v_4v_2\rho^2-\frac{v_4^2}{2}\rho^2-\frac{v_1}{2}\rho^2-\frac{v_2}{2}\rho^2+\frac{v_4}{2}\rho^2)$

We have several arrangements,

\begin{enumerate}
\item 
$v_1+v_2\overset{d}{\geq}v_4\overset{c}{>}v_3\overset{b}{>}{v_2}\overset{a}{>}v_1\overset{e}{\geq}{0}$

But $v_1+v_2-d-c-b=v_2\Rightarrow{v_1=v_1+v_2-v_2=b+c+d}$

Thus, we substitute 
$v_1\rightarrow{b+c+d}$, $v_2\rightarrow{a+b+c+d}$, $v_3\rightarrow{a+2b+c+d}$, $v_4\rightarrow{a+2b+2c+d}$, and compute series with the new variables as indices, where $d\geq{0}$ and $a,b,c\geq{1}$

\item 
$v_1+v_2\overset{d}{\geq}v_4\overset{c}{>}v_2\overset{b}{\geq}{v_3}\overset{a}{>}v_1\overset{e}{\geq}{0}$

But $v_1+v_2-d-c=v_2\Rightarrow{v_1=v_1+v_2-v_2=c+d}$

Thus, we substitute 
$v_1\rightarrow{c+d}$, $v_2\rightarrow{a+b+c+d}$, $v_3\rightarrow{a+c+d}$, $v_4\rightarrow{a+b+2c+d}$, and compute series with the new variables as indices, where $b,d\geq{0}$ and $a,c\geq{1}$

\item 
$v_1+v_2\overset{d}{\geq}v_4\overset{c}{>}v_3\overset{b}{>}{v_1}\overset{a}{\geq}v_2\overset{e}{\geq}{0}$

But $v_1+v_2-d-c-b=v_1\Rightarrow{v_2=v_1+v_2-v_1=b+c+d}$

Thus, we substitute 
$v_1\rightarrow{a+b+c+d}$, $v_2\rightarrow{b+c+d}$, $v_3\rightarrow{a+2b+c+d}$, $v_4\rightarrow{a+2b+2c+d}$, and compute series with the new variables as indices, where $a,d\geq{0}$ and $b,c\geq{1}$

\item 
$v_1+v_2\overset{d}{\geq}v_3\overset{c}{\geq}v_4\overset{b}{>}{v_2}\overset{a}{>}v_1\overset{e}{\geq}{0}$

But $v_1+v_2-d-c-b=v_2\Rightarrow{v_1=v_1+v_2-v_2=b+c+d}$

Thus, we substitute 
$v_1\rightarrow{b+c+d}$, $v_2\rightarrow{a+b+c+d}$, $v_3\rightarrow{a+2b+2c+d}$, $v_4\rightarrow{a+2b+c+d}$, and compute series with the new variables as indices, where $c,d\geq{0}$ and $a,b\geq{1}$
\item 
$v_1+v_2\overset{d}{>}v_3\overset{c}{\geq}v_4\overset{b}{>}{v_1}\overset{a}{\geq}v_2\overset{e}{\geq}{0}$

But $v_1+v_2-d-c-b=v_1\Rightarrow{v_2=v_1+v_2-v_1=b+c+d}$

Thus, we substitute 
$v_1\rightarrow{a+b+c+d}$, $v_2\rightarrow{b+c+d}$, $v_3\rightarrow{a+2b+2c+d}$, $v_4\rightarrow{a+2b+c+d}$, and compute series with the new variables as indices, where $a,c\geq{0}$ and $b,d\geq{1}$
\item 
$v_3\overset{d}{\geq}v_1+v_2\overset{c}{\geq}v_4\overset{b}{>}{v_2}\overset{a}{>}v_1\overset{e}{\geq}{0}$

But $v_1+v_2-c-b=v_2\Rightarrow{v_1=v_1+v_2-v_2=b+c}$

Thus, we substitute 
$v_1\rightarrow{b+c}$, 
$v_2\rightarrow{a+b+c}$, 
$v_3\rightarrow{a+2b+2c+d}$, 
$v_4\rightarrow{a+2b+c}$, and compute series with the new variables as indices, where $c,d\geq{0}$ and $a,b\geq{1}$
\item 
$v_3\overset{d}{\geq}v_1+v_2\overset{c}{\geq}v_4\overset{b}{>}{v_1}\overset{a}{\geq}v_2\overset{e}{\geq}{0}$

But $v_1+v_2-c-b=v_1\Rightarrow{v_2=v_1+v_2-v_1=b+c}$

Thus, we substitute 
$v_1\rightarrow{a+b+c}$, 
$v_2\rightarrow{b+c}$, 
$v_3\rightarrow{a+2b+2c+d}$, 
$v_4\rightarrow{a+2b+c}$, and compute series with the new variables as indices, where $a,c,d\geq{0}$ and $b\geq{1}$
\end{enumerate}
\section{Case 4}
$v_4>v_1\geq{v_3}\geq{0}$

$v_4>v_2\geq{0}$

$\Rightarrow{v_{11}}\geq{-v_2-v_3}$

$\Rightarrow\alpha:=\min\{v_2,v_2+v_{11}+v_4\}=\begin{cases}
       v_2, & v_{11}\geq{-v_4}\\
       v_2-1,v_2-2,\dots, & v_{11}<{-v_4}\\
     \end{cases}$

     $\Rightarrow{f(p,t)=p^{7v_1+10v_2+11v_3+7v_4+v_1}t^{4v_1+6v_2+6v_3+4v_4}=p^{8v_1+10v_2+11v_3+7v_4}t^{4v_1+6v_2+6v_3+4v_4}}$

We have two sub cases

\subsection{Sub case 4.1}
$-v_4<-v_2-v_3\Rightarrow{v_4>v_2+v_3}$

There is no phase transition here, since $v_{11}\geq{-v_2-v_3}>-v_4$

For $v_{11}\geq{-v_2}$, we have $p^{\min}(1+\alpha\rho)\mu(a_{11})=p^{v_2}(1+v_2\rho).$

For $-v_2-v_3\leq{v_{11}}\leq{-v_2-1}$, we have $p^{\min}(1+\alpha\rho)\mu(a_{11})=\sum_{-v_2-v_3}^{-v_2-1}p^{v_2}\rho(1+v_2\rho)=p^{v_2}v_3\rho(1+v_2\rho)=p^{v_2}v_3\rho+p^{v_2}v_2v_3\rho^2.$

So we have $\sum_{v_{11}\geq{-v_2-v_3}}p^{\min}(1+\alpha\rho)\mu(a_{11})=p^{v_2}(1+v_2\rho+v_3\rho+v_2v_3\rho^2).$

We have several arrangements,
\begin{enumerate}
\item 
$v_4\overset{d}{>}v_2+v_3\overset{c}{\geq}v_1\overset{b}{\geq}{v_3}\overset{a}{>}v_2\overset{e}{\geq}{0}$

But $v_2+v_3-c-b=v_3\Rightarrow{v_2=v_2+v_3-v_3=b+c}$

Thus, we substitute 
$v_1\rightarrow{a+2b+c}$, 
$v_2\rightarrow{b+c}$, 
$v_3\rightarrow{a+b+c}$, 
$v_4\rightarrow{a+2b+2c+d}$, and compute series with the new variables as indices, where $b,c\geq{0}$ and $a,d\geq{1}$

\item 
$v_4\overset{d}{>}v_2+v_3\overset{c}{\geq}v_1\overset{b}{\geq}{v_2}\overset{a}{\geq}v_3\overset{e}{\geq}{0}$

But $v_2+v_3-c-b=v_2\Rightarrow{v_3=v_2+v_3-v_2=b+c}$

Thus, we substitute 
$v_1\rightarrow{a+2b+c}$, 
$v_2\rightarrow{a+b+c}$, 
$v_3\rightarrow{b+c}$, 
$v_4\rightarrow{a+2b+2c+d}$, and compute series with the new variables as indices, where $a,b,c\geq{0}$ and $d\geq{1}$.
\item 
$v_4\overset{d}{>}v_2+v_3\overset{a}{\geq}v_2\overset{c}{>}{v_1}\overset{b}{\geq}v_3\overset{a}{\geq}{0}$


Thus, we substitute 
$v_1\rightarrow{a+b}$, 
$v_2\rightarrow{a+b+c}$, 
$v_3\rightarrow{a}$, 
$v_4\rightarrow{2a+b+c+d}$, and compute series with the new variables as indices, where $a,b\geq{0}$ and $c,d\geq{1}$.

\item 
$v_4\overset{d}{>}v_1\overset{c}{\geq}v_2+v_3\overset{a}{\geq}{v_2}\overset{b}{\geq}v_3\overset{a}{\geq}{0}$

Thus, we substitute 
$v_1\rightarrow{2a+b+c}$, 
$v_2\rightarrow{a+b}$, 
$v_3\rightarrow{a}$, 
$v_4\rightarrow{2a+b+c+d}$, and compute series with the new variables as indices, where $a,b,c\geq{0}$ and $d\geq{1}$.

\item 
$v_4\overset{d}{>}v_1\overset{c}{\geq}v_2+v_3\overset{a}{\geq}{v_3}\overset{b}{>}v_2\overset{a}{\geq}{0}$

Thus, we substitute 
$v_1\rightarrow{2a+b+c}$, 
$v_2\rightarrow{a}$, 
$v_3\rightarrow{a+b}$, 
$v_4\rightarrow{2a+b+c+d}$, and compute series with the new variables as indices, where $a,c\geq{0}$ and $b,d\geq{1}.$
\end{enumerate}
@@@@ CHECKED @@@@
\subsection{Sub case 4.2}
$-v_2-v_3<{-v_4}\Rightarrow{v_2+v_3>{v_4}}$

For $v_{11}\geq{-v_2}$, we have $p^{\min}(1+\alpha\rho)\mu(a_{11})=p^{v_2}(1+v_2\rho).$

For $-v_4\leq{v_{11}}\leq{-v_2-1}$, we have $p^{\min}(1+\alpha\rho)\mu(a_{11})=\sum_{-v_4}^{-v_2-1}p^{v_2}\rho(1+v_2\rho)=p^{v_2}(v_4-v_2)\rho(1+v_2\rho)=p^{v_2}(v_4-v_2)\rho+p^{v_2}v_2(v_4-v_2)\rho^2.$

For $-v_2-v_3\leq{v_{11}}\leq{-v_4-1}$, we have $p^{\min}(1+\alpha\rho)\mu(a_{11})=\sum_{-v_2-v_3}^{-v_4-1}p^{v_2}\rho(1+\alpha\rho)=\sum_{i=1}^{v_2+v_3-v_4}p^{v_2}\rho(1+(v_2-i)\rho)=p^{v_2}(v_2+v_3-v_4)\rho+(v_2+v_3-v_4)v_2\rho^2-\binom{v_2+v_3-v_4+1}{2}\rho^2.$

So we have $\sum_{v_{11}\geq{-v_2-v_3}}p^{\min}(1+\alpha\rho)\mu(a_{11})=p^{v_2}(1+v_2\rho+(v_4-v_2))\rho+v_2(v_4-v_2)\rho^2+(v_2+v_3-v_4)\rho+(v_2+v_3-v_4)v_2\rho^2-\frac{(v_2+v_3-v_4+1)(v_2+v_3-v_4)}{2}\rho^2)=p^{v_2}(1+v_2v_4\rho^2+v_2\rho+v_3\rho+v_3v_2\rho^2-v_4v_2\rho^2-\frac{v_2^2}{2}\rho^2-v_2v_3\rho^2+v_2v_4\rho^2-\frac{v_3^2}{2}\rho^2+v_3v_4\rho^2-\frac{v_4^2}{2}\rho^2-\frac{v_2}{2}\rho^2-\frac{v_3}{2}\rho^2+\frac{v_4}{2}\rho^2)$.

We have several arrangements,
\begin{enumerate}
\item 
$v_2+v_3\overset{d}{\geq}v_4\overset{c}{>}v_1\overset{b}{\geq}{v_2}\overset{a}{\geq}v_3\overset{e}{\geq}{0}$

But $v_2+v_3-d-c-b=v_2\Rightarrow{v_3=v_2+v_3-v_2=b+c+d}$

Thus, we substitute 
$v_1\rightarrow{a+2b+c+d}$, 
$v_2\rightarrow{a+b+c+d}$, 
$v_3\rightarrow{b+c+d}$, 
$v_4\rightarrow{a+2b+2c+d}$, and compute series with the new variables as indices, where $a,b,d\geq{0}$ and $c\geq{1}$

\item 
$v_2+v_3\overset{d}{>}v_4\overset{c}{>}v_1\overset{b}{\geq}{v_3}\overset{a}{>}v_2\overset{e}{\geq}{0}$

But $v_2+v_3-d-c-b=v_3\Rightarrow{v_2=v_2+v_3-v_3=b+c+d}$

Thus, we substitute 
$v_1\rightarrow{a+2b+c+d}$, 
$v_2\rightarrow{b+c+d}$, 
$v_3\rightarrow{a+b+c+d}$, 
$v_4\rightarrow{a+2b+2c+d}$, and compute series with the new variables as indices, where $b\geq{0}$ and $a,c,d\geq{1}$
\item 
$v_2+v_3\overset{d}{\geq}v_4\overset{c}{>}v_2\overset{b}{>}{v_1}\overset{a}{\geq}v_3\overset{e}{\geq}{0}$

But $v_2+v_3-d-c=v_2\Rightarrow{v_3=v_2+v_3-v_2=c+d}$

Thus, we substitute 
$v_1\rightarrow{a+c+d}$, 
$v_2\rightarrow{a+b+c+d}$, 
$v_3\rightarrow{c+d}$, 
$v_4\rightarrow{a+b+2c+d}$, and compute series with the new variables as indices, where $a,d\geq{0}$ and $b,c\geq{1}$

\end{enumerate}

\section{Case 5}
$v_2\geq{v_4}>v_1>v_3\geq{0}$

$\Rightarrow{v_{11}}\geq{-v_2-v_3}$

$\Rightarrow\alpha:=\min\{v_4,v_2+v_{11}+v_4\}=\begin{cases}
       v_4, & v_{11}\geq{-v_2}\\
       v_4-1,v_4-2,\dots, & v_{11}<{-v_2}\\
     \end{cases}$

     $\Rightarrow{f(p,t)=p^{7v_1+10v_2+11v_3+7v_4+v_1}t^{4v_1+6v_2+6v_3+4v_4}=p^{8v_1+10v_2+11v_3+7v_4}t^{4v_1+6v_2+6v_3+4v_4}}$

For $v_{11}\geq{-v_2}$, we have $p^{\min}(1+\alpha\rho)\mu(a_{11})=p^{v_2}(1+v_4\rho).$

For $-v_2-v_3\leq{v_{11}}\leq{-v_2-1}$, we have $p^{\min}(1+\alpha\rho)\mu(a_{11})=\sum_{-v_2-v_3}^{-v_2-1}p^{v_2}\rho(1+\alpha\rho)=\sum_{i=1}^{v_3}p^{v_2}\rho(1+(v_4-i)\rho)=p^{v_2}(v_3\rho+v_3v_4\rho^2-\binom{v_3+1}{2}\rho^2).$

So we have $\sum_{v_{11}\geq{-v_2-v_3}}p^{\min}(1+\alpha\rho)\mu(a_{11})=p^{v_2}(1+v_4\rho+v_3\rho+v_3v_4\rho^2-\frac{(v_3+1)v_3}{2}\rho^2)=p^{v_2}(1+v_4\rho+v_3\rho+v_3v_4\rho^2-\frac{v_3^2}{2}\rho^2-\frac{v_3}{2}\rho^2).$

$v_2\overset{d}{\geq}v_4\overset{c}{>}v_1\overset{b}{\geq}{v_3}\overset{a}{\geq}{0}$

Thus, we substitute 
$v_1\rightarrow{a+b}$, 
$v_2\rightarrow{a+b+c+d}$, 
$v_3\rightarrow{a}$, 
$v_4\rightarrow{a+b+c}$, and compute series with the new variables as indices, where $a,b,d\geq{0}$ and $c\geq{1}$

\section{Case 6}
$v_2\geq{v_4}>v_1\geq{0}$

$v_3>v_1\geq{0}$

$\Rightarrow{v_{11}}\geq{-v_2-v_1}$

$\Rightarrow\alpha:=\min\{v_4,v_2+v_{11}+v_4\}=\begin{cases}
       v_4, & v_{11}\geq{-v_2}\\
       v_4-1,v_4-2,\dots, & v_{11}<{-v_2}\\
     \end{cases}$

     $\Rightarrow{f(p,t)=p^{7v_1+10v_2+11v_3+7v_4+v_1}t^{4v_1+6v_2+6v_3+4v_4}=p^{8v_1+10v_2+11v_3+7v_4}t^{4v_1+6v_2+6v_3+4v_4}}$

For $v_{11}\geq{-v_2}$, we have $p^{\min}(1+\alpha\rho)\mu(a_{11})=p^{v_2}(1+v_4\rho).$

For $-v_2-v_1\leq{v_{11}}\leq{-v_2-1}$, we have $p^{\min}(1+\alpha\rho)\mu(a_{11})=\sum_{-v_2-v_1}^{-v_2-1}p^{v_2}\rho(1+\alpha\rho)=\sum_{i=1}^{v_1}p^{v_2}\rho(1+(v_4-i)\rho)=p^{v_2}(v_1\rho+v_1v_4\rho^2-\binom{v_1+1}{2}\rho^2).$

So we have $\sum_{v_{11}\geq{-v_2-v_1}}p^{\min}(1+\alpha\rho)\mu(a_{11})=p^{v_2}(1+v_4\rho+v_1\rho+v_1v_4\rho^2-\frac{(v_1+1)v_1}{2}\rho^2)=p^{v_2}(1+v_4\rho+v_1\rho+v_1v_4\rho^2-\frac{v_1^2}{2}\rho^2-\frac{v_1}{2}\rho^2).$

We have several arrangements,
\begin{enumerate}
    \item 
$v_2\overset{d}{\geq}v_4\overset{c}{>}v_3\overset{b}{>}{v_1}\overset{a}{\geq}{0}$

Thus, we substitute $v_1\rightarrow{a}$, $v_2\rightarrow{a+b+c+d}$, $v_3\rightarrow{a+b}$, $v_4\rightarrow{a+b+c}$, and compute series with the new variables as indices, where $a,d\geq{0}$ and $b,c\geq{1}$
    \item 
$v_2\overset{d}{\geq}v_3\overset{c}{\geq}v_4\overset{b}{>}{v_1}\overset{a}{\geq}{0}$

Thus, we substitute $v_1\rightarrow{a}$, $v_2\rightarrow{a+b+c+d}$, $v_3\rightarrow{a+b+c}$, $v_4\rightarrow{a+b}$, and compute series with the new variables as indices, where $a,c,d\geq{0}$ and $b\geq{1}$
    \item 
$v_3\overset{d}{>}v_2\overset{c}{\geq}v_4\overset{b}{>}{v_1}\overset{a}{\geq}{0}$

Thus, we substitute $v_1\rightarrow{a}$, $v_2\rightarrow{a+b+c}$, $v_3\rightarrow{a+b+c+d}$, $v_4\rightarrow{a+b}$, and compute series with the new variables as indices, where $a,c\geq{0}$ and $b,d\geq{1}$

\end{enumerate}

\section{Case 7}
$v_2\geq{v_4}\geq{0}$

$v_3>v_1\geq{v_4}\geq{0}$

$\Rightarrow{v_{11}}\geq{-v_2-v_1}$

$\Rightarrow{f(p,t)=p^{7v_1+10v_2+11v_3+7v_4+v_4}t^{4v_1+6v_2+6v_3+4v_4}=p^{7v_1+10v_2+11v_3+8v_4}t^{4v_1+6v_2+6v_3+4v_4}}$

$\Rightarrow\alpha:=\min\{v_4,v_2+v_{11}+v_1\}=\begin{cases}
       v_4, & v_{11}\geq{v_4-v_1-v_2}\\
       v_4-1,v_4-2,\dots, & v_{11}<{v_4-v_1-v_2}\\
     \end{cases}$

There are no two sub cases here, because the phase transition occurs at $v_{11}={v_4-v_1-v_2-1}$, thus 

if $v_4=0$ then the transition would be at $v_{11}=-v_2-v_1-1<-v_2-v_1$, which is a contradiction. 

For $v_4\geq{1}$ the transition would be at $a_{11}\geq{-v_2-v_1}$, which is always true for this case.

For $v_{11}\geq{-v_2}$, we have $p^{\min}(1+\alpha\rho)\mu(a_{11})=p^{v_2}(1+v_4\rho).$

For $v_4-v_1-v_2\leq{v_{11}}\leq{-v_2-1}$, we have $p^{\min}(1+\alpha\rho)\mu(a_{11})=\sum_{v_4-v_1-v_2}^{-v_2-1}p^{v_2}\rho(1+v_4\rho)=\sum_{i=1}^{v_1-v_4}p^{v_2}\rho(1+v_4\rho)=p^{v_2}(v_1-v_4)\rho(1+v_4\rho)=p^{v_2}(v_1-v_4)\rho+p^{v_2}(v_1-v_4)v_4\rho^2.$

For $-v_1-v_2\leq{v_{11}}\leq{v_4-v_1-v_2-1}$, we have $p^{\min}(1+\alpha\rho)\mu(a_{11})=\sum_{-v_1-v_2}^{v_4-v_1-v_2-1}p^{v_2}\rho(1+\alpha\rho)=\sum_{i=1}^{v_4}p^{v_2}\rho(1+(v_4-i)\rho)=p^{v_2}v_4\rho+p^{v_2}v_4^2\rho^2-p^{v_2}\binom{v_4+1}{2}\rho^2.$

So we have $\sum_{v_{11}\geq{-v_2-v_1}}p^{\min}\mu(a_{11})=p^{v_2}(1+v_4\rho+(v_4-v_1)\rho+(v_4-v_1)v_4\rho^2+v_4\rho+v_4^2\rho^2-\frac{v_4(v_4-1)}{2}\rho^2)=p^{v_2}(1+3v_4\rho-v_1\rho+2v_4^2\rho^2-v_1v_4\rho^2-\frac{v_4^2}{2}\rho^2+\frac{v_4}{2}\rho^2)$

We have several arrangements,
\begin{enumerate}
    \item 
$v_2\overset{d}{\geq}v_3\overset{c}{>}v_1\overset{b}{\geq}{v_4}\overset{a}{\geq}{0}$

Thus, we substitute $v_1\rightarrow{a+b}$, $v_2\rightarrow{a+b+c+d}$, $v_3\rightarrow{a+b+c}$, $v_4\rightarrow{a}$, and compute series with the new variables as indices, where $a,b,d\geq{0}$ and $c\geq{1}$    
\item 
$v_3\overset{d}{>}v_2\overset{c}{>}v_1\overset{b}{\geq}{v_4}\overset{a}{\geq}{0}$

Thus, we substitute $v_1\rightarrow{a+b}$, $v_2\rightarrow{a+b+c}$, $v_3\rightarrow{a+b+c+d}$, $v_4\rightarrow{a}$, and compute series with the new variables as indices, where $a,b\geq{0}$ and $c,d\geq{1}$
    \item 
$v_3\overset{d}{>}v_1\overset{c}{\geq}v_2\overset{b}{\geq}{v_4}\overset{a}{\geq}{0}$

Thus, we substitute $v_1\rightarrow{a+b+c}$, $v_2\rightarrow{a+b}$, $v_3\rightarrow{a+b+c+d}$, $v_4\rightarrow{a}$, and compute series with the new variables as indices, where $a,b,c\geq{0}$ and $d\geq{1}$

\end{enumerate}
\section{Case 8}
$v_2\geq{v_4}\geq{0}$

$v_1\geq{v_4}\geq{0}$

$v_1\geq{v_3}\geq{0}$

$\Rightarrow{v_{11}}\geq{-v_2-v_3}$

$\Rightarrow\alpha:=\min\{v_4,v_2+v_{11}+v_1\}=\begin{cases}
       v_4, & v_{11}\geq{v_4-v_1-v_2}\\
       v_4-1,v_4-2,\dots, & v_{11}<{v_4-v_1-v_2}\\
     \end{cases}$

     $\Rightarrow{f(p,t)=p^{7v_1+10v_2+11v_3+7v_4+v_4}t^{4v_1+6v_2+6v_3+4v_4}=p^{7v_1+10v_2+11v_3+8v_4}t^{4v_1+6v_2+6v_3+4v_4}}$

There are two sub cases here

\subsection{Sub case 8.1}

$-v_2-v_3\geq{v_4-v_1-v_2}\Rightarrow{-v_3\geq{v_4-v_1}}\Rightarrow{v_1\geq{v_3+v_4}}$

For $v_{11}\geq{-v_2}$, we have $p^{\min}(1+\alpha\rho)\mu(a_{11})=p^{v_2}(1+v_4\rho).$

For $-v_2-v_3\leq{v_{11}}\leq{-v_2-1}$, we have $p^{\min}(1+\alpha\rho)\mu(a_{11})=\sum_{-v_2-v_3}^{-v_2-1}p^{v_2}\rho(1+v_4\rho)=\sum_{i=1}^{v_3}p^{v_2}\rho(1+v_4\rho)=p^{v_2}(v_3\rho+v_3v_4\rho^2).$

So we have $\sum_{v_{11}\geq{-v_2-v_3}}p^{\min}(1+\alpha\rho)\mu(a_{11})=p^{v_2}(1+v_4\rho+v_3\rho+v_3v_4\rho^2).$

We have several arrangements,
\begin{enumerate}
    \item 
$v_1\overset{d}{\geq}v_3+v_4\overset{a}{\geq}v_3\overset{c}{>}{v_2}\overset{b}{\geq}v_4\overset{a}{\geq}{0}$

But $e=v_2+v_3-v_3=v_2=a+b.$

Thus, we substitute 
$v_1\rightarrow{2a+b+c+d}$, 
$v_2\rightarrow{a+b}$, 
$v_3\rightarrow{a+b+c}$, 
$v_4\rightarrow{a}$, and compute series with the new variables as indices, where $a,b,d\geq{0}$ and $c\geq{1}$  
    \item 
$v_1\overset{d}{\geq}v_3+v_4\overset{c}{\geq}v_2\overset{b}{\geq}{v_3}\overset{a}{\geq}v_4\overset{e}{\geq}{0}$

But $v_3=v_3+v_4-c-b\Rightarrow{v_4=b+c}$

Thus, we substitute 
$v_1\rightarrow{a+2b+2c+d}$, 
$v_2\rightarrow{a+2b+c}$, 
$v_3\rightarrow{a+b+c}$, 
$v_4\rightarrow{b+c}$, and compute series with the new variables as indices, where $a,b,c,d\geq{0}.$

    \item 
$v_1\overset{d}{\geq}v_3+v_4\overset{c}{\geq}v_2\overset{b}{\geq}{v_4}\overset{a}>v_3\overset{e}{\geq}{0}$

Thus, we substitute 
$v_1\rightarrow{a+2b+2c+d}$, 
$v_2\rightarrow{a+2b+c}$, 
$v_3\rightarrow{a+b+c}$, 
$v_4\rightarrow{b+c}$, and compute series with the new variables as indices, where $b,c,d\geq{0}$ and $a\geq{1}$
    \item 
$v_1\overset{d}{\geq}v_2\overset{c}>v_3+v_4\overset{a}{\geq}{v_4}\overset{b}>v_3\overset{a}{\geq}{0}$

Thus, we substitute 
$v_1\rightarrow{2a+b+c+d}$, 
$v_2\rightarrow{2a+b+c}$, 
$v_3\rightarrow{a}$, 
$v_4\rightarrow{a+b}$, and compute series with the new variables as indices, where $a,d\geq{0}$ and $b,c\geq{1}$
    \item 
$v_1\overset{d}{\geq}v_2\overset{c}>v_3+v_4\overset{a}{\geq}{v_3}\overset{b}\geq{v_4}\overset{a}{\geq}{0}$

Thus, we substitute 
$v_1\rightarrow{2a+b+c+d}$, 
$v_2\rightarrow{2a+b+c}$, 
$v_3\rightarrow{a+b}$, 
$v_4\rightarrow{a}$, and compute series with the new variables as indices, where $a,b,d\geq{0}$ and $c\geq{1}$
\item 
$v_2\overset{d}>v_1\overset{c}{\geq}v_3+v_4\overset{a}{\geq}{v_3}\overset{b}\geq{v_4}\overset{a}{\geq}{0}$

Thus, we substitute 
$v_1\rightarrow{2a+b+c}$, 
$v_2\rightarrow{2a+b+c+d}$, 
$v_3\rightarrow{a+b}$, 
$v_4\rightarrow{a}$, and compute series with the new variables as indices, where $a,b,c\geq{0}$ and $d\geq{1}$
\item 
$v_2\overset{d}>v_1\overset{c}{\geq}v_3+v_4\overset{a}{\geq}{v_4}\overset{b}>{v_3}\overset{a}{\geq}{0}$

Thus, we substitute 
$v_1\rightarrow{2a+b+c}$, 
$v_2\rightarrow{2a+b+c+d}$, 
$v_3\rightarrow{a}$, 
$v_4\rightarrow{a+b}$, and compute series with the new variables as indices, where $a,c\geq{0}$ and $b,d\geq{1}$
\end{enumerate}

\subsection{Sub case 8.2}

$-v_2-v_3<{v_4-v_1-v_2}\Rightarrow{-v_3<{v_4-v_1}}\Rightarrow{v_1<{v_3+v_4}}$

For $v_{11}\geq{-v_2}$, we have $p^{\min}(1+\alpha\rho)\mu(a_{11})=p^{v_2}(1+v_4\rho).$

For $v_4-v_1-v_2\leq{v_{11}}\leq{-v_2-1}$, we have $p^{\min}(1+\alpha\rho)\mu(a_{11})=\sum_{v_4-v_1-v_2}^{-v_2-1}p^{v_2}\rho(1+v_4\rho)=p^{v_2}((v_1-v_4)\rho+(v_1-v_4)v_4\rho^2).$

For $-v_2-v_3\leq{v_{11}}\leq{v_4-v_1-v_2-1}$, we have $p^{\min}(1+\alpha\rho)\mu(a_{11})=\sum_{-v_2-v_3}^{v_4-v_1-v_2-1}p^{v_2}\rho(1+\alpha\rho)=\sum_{i=1}^{v_3+v_4-v_1}p^{v_2}\rho(1+(v_4-i))\rho)=p^{v_2}((v_3+v_4-v_1)\rho+(v_3+v_4-v_1)v_4\rho^2-\binom{v_3+v_4-v_1+1}{2}\rho^2).$

So we have $\sum_{v_{11}\geq{-v_2-v_3}}\rho(1+\alpha\rho)=p^{v_2}(
1+v_4\rho+(v_1-v_4)\rho+(v_1-v_4)v_4\rho^2+
(v_3+v_4-v_1)\rho+(v_3+v_4-v_1)v_4\rho^2-\frac{(v_3+v_4-v_1+1)(v_3+v_4-v_1)}{2}\rho^2)=p^{v_2}(1+v_3\rho+v_4\rho-\frac{v_3^2}{2}\rho^2+v_1v_3\rho^2-\frac{v_4^2}{2}\rho^2+v_1v_4\rho^2-\frac{v_1^2}{2}\rho^2-v_3\rho^2-v_4\rho^2+v_1\rho^2)$.

We have several arrangements,
\begin{enumerate}
    \item 
$v_3+v_4\overset{d}{>}v_1\overset{c}{\geq}v_3\overset{b}{>}{v_2}\overset{a}{\geq}v_4\overset{e}{\geq}{0}$

But $v_3+v_4-d-c=v_3\Rightarrow{v_4=c+d}.$

Thus, we substitute $v_1\rightarrow{a+b+2c+d}$, $v_2\rightarrow{a+c+d}$, $v_3\rightarrow{a+b+c+d}$, $v_4\rightarrow{c+d}$, and compute series with the new variables as indices, where $a,c\geq{0}$ and $b,d\geq{1}$  
    \item 
$v_3+v_4\overset{d}{>}v_1\overset{c}{\geq}v_2\overset{b}{\geq}{v_3}\overset{a}{\geq}v_4\overset{e}{\geq}{0}$

But $v_3+v_4-d-c-b=v_3\Rightarrow{v_4=b+c+d}.$

Thus, we substitute $v_1\rightarrow{a+2b+2c+d}$, $v_2\rightarrow{a+2b+c+d}$, $v_3\rightarrow{a+b+c+d}$, $v_4\rightarrow{b+c+d}$, and compute series with the new variables as indices, where $a,b,c\geq{0}$ and $d\geq{1}$.  
    \item 
$v_3+v_4\overset{d}{>}v_1\overset{c}{\geq}v_2\overset{b}{\geq}{v_4}\overset{a}{>}v_3\overset{e}{\geq}{0}$

But $v_3+v_4-d-c-b=v_4\Rightarrow{v_3=b+c+d}.$

Thus, we substitute $v_1\rightarrow{a+2b+2c+d}$, $v_2\rightarrow{a+2b+c+d}$, $v_3\rightarrow{b+c+d}$, $v_4\rightarrow{a+b+c+d}$, and compute series with the new variables as indices, where $b,c\geq{0}$ and $a,d\geq{1}$
    \item 
$v_3+v_4\overset{d}{\geq}v_2\overset{c}{>}v_1\overset{b}{\geq}{v_4}\overset{a}{>}v_3\overset{e}{\geq}{0}$

But $v_3+v_4-d-c-b=v_4\Rightarrow{v_3=b+c+d}.$

Thus, we substitute $v_1\rightarrow{a+2b+c+d}$, $v_2\rightarrow{a+2b+2c+d}$, $v_3\rightarrow{b+c+d}$, $v_4\rightarrow{a+b+c+d}$, and compute series with the new variables as indices, where $b,d\geq{0}$ and $a,c\geq{1}$
    \item 
$v_3+v_4\overset{d}>v_2\overset{c}{>}v_1\overset{b}{\geq}{v_3}\overset{a}{\geq}v_4\overset{e}{\geq}{0}$

But $v_3+v_4-d-c-b=v_3\Rightarrow{v_4=b+c+d}.$

Thus, we substitute $v_1\rightarrow{a+2b+c+d}$, $v_2\rightarrow{a+2b+2c+d}$, $v_3\rightarrow{a+b+c+d}$, $v_4\rightarrow{b+c+d}$, and compute series with the new variables as indices, where $a,b\geq{0}$ and $c,d\geq{1}$
    \item 
$v_2\overset{d}{>}v_3+v_4\overset{c}{>}v_1\overset{b}{\geq}{v_4}\overset{a}{>}v_3\overset{e}{\geq}{0}$

But $v_3+v_4-c-b=v_4\Rightarrow{v_3=b+c}.$

Thus, we substitute $v_1\rightarrow{a+2b+c}$, $v_2\rightarrow{a+2b+2c+d}$, $v_3\rightarrow{b+c}$, $v_4\rightarrow{a+b+c}$, and compute series with the new variables as indices, where $b,d\geq{0}$ and $a,c\geq{1}$
    \item 
$v_2\overset{d}{\geq}v_3+v_4\overset{c}{>}v_1\overset{b}{\geq}{v_3}\overset{a}{\geq}v_4\overset{e}{\geq}{0}$

But $v_3+v_4-c-b=v_3\Rightarrow{v_4=b+c}.$

Thus, we substitute $v_1\rightarrow{a+2b+c}$, $v_2\rightarrow{a+2b+2c+d}$, $v_3\rightarrow{a+b+c}$, $v_4\rightarrow{b+c}$, and compute series with the new variables as indices, where $a,b,d\geq{0}$ and $c\geq{1}$
\end{enumerate}

Checking all the cases by the $4!$ arrangements.

\begin{enumerate}

    \item $v_1\geq{v_2}\geq{v_3}\geq{v_4}\geq{0}$

    $v_1\geq{v_3+v_4}\geq{v_2}\geq{v_3}\geq{v_4}\geq{0}$ (8.1.2)
    
    $v_1\geq{v_2}>v_3+v_4\geq{v_3}\geq{v_4}\geq{0}$ (8.1.5)
    
    $v_3+v_4>v_1\geq{v_2}\geq{v_3}\geq{v_4}\geq{0}$ (8.2.2)

    \item $v_1\geq{v_2}\geq{v_4}>v_3\geq{0}$

    $v_1\geq{v_3+v_4}\geq{v_2}\geq{v_4}>v_3\geq{0}$ (8.1.3)
    
    $v_1\geq{v_2}>v_3+v_4\geq{v_4}>v_3\geq{0}$ (8.1.4)
    
    $v_3+v_4>v_1\geq{v_2}\geq{v_4}>v_3\geq{0}$ (8.2.3)

    \item $v_1\geq{v_3}>v_2\geq{v_4}\geq{0}$

    $v_1\geq{v_3+v_4}\geq{v_3}>v_2\geq{v_4}\geq{0}$ (8.1.1)
    
    $v_3+v_4>v_1\geq{v_3}>v_2\geq{v_4}\geq{0}$ (8.2.1)

    \item $v_1\geq{v_3}\geq{v_4}>v_2\geq{0}$

$v_1\geq{v_2+v_3}\geq{v_3}\geq{v_4}>v_2\geq{0}$ (2.1.1)

$v_2+v_3>v_1\geq{v_3}\geq{v_4}>v_2\geq{0}$ (2.2.1)

    \item $v_1\geq{v_4}>v_2\geq{v_3}\geq{0}$

    $v_1\geq{v_2+v_3}\geq{v_4}>v_2\geq{v_3}\geq{0}$ (2.1.3)

    $v_1\geq{v_4}>v_2+v_3\geq{v_2}\geq{v_3}\geq{0}$ (2.1.4)

    $v_2+v_3>v_1\geq{v_4}>v_2\geq{v_3}\geq{0}$ (2.2.3)
    
\item $v_1\geq{v_4}>v_3>v_2\geq{0}$

    $v_1\geq{v_2+v_3}\geq{v_4}>v_3>v_2\geq{0}$ (2.1.2)

    $v_2+v_3>v_1\geq{v_4}>v_3>v_2\geq{0}$ (2.2.2)

    $v_1\geq{v_4}>v_2+v_3\geq{v_3}>v_2\geq{0}$ (2.1.5)

    \item $v_2>v_1\geq{v_3}\geq{v_4}\geq{0}$

    $v_2>v_1\geq{v_3+v_4}\geq{v_3}\geq{v_4}\geq{0}$ (8.1.6)

    $v_2\geq{v_3+v_4}>v_1\geq{v_3}\geq{v_4}\geq{0}$ (8.2.7)

    $v_3+v_4>{v_2}>v_1\geq{v_3}\geq{v_4}\geq{0}$ (8.2.5)

    \item $v_2>v_1\geq{v_4}>v_3\geq{0}$

    $v_2>v_1\geq{v_3+v_4}\geq{v_4}>v_3\geq{0}$ (8.1.7)

    $v_2>v_3+v_4>v_1\geq{v_4}>v_3\geq{0}$ (8.2.6)

    $v_3+v_4\geq{v_2}>v_1\geq{v_4}>v_3\geq{0}$ (8.2.4)

    \item $v_2\geq{v_3}>v_1\geq{v_4}\geq{0}$ (7.1)
    \item $v_2\geq{v_3}\geq{v_4}>v_1\geq{0}$ (6.2)
    \item $v_2\geq{v_4}>v_1\geq{v_3}\geq{0}$ (5)
    \item $v_2\geq{v_4}>v_3>v_1\geq{0}$ (6.1)
    \item $v_3>v_1\geq{v_2}\geq{v_4}\geq{0}$ (7.3)
    \item $v_3>v_1\geq{v_4}>v_2\geq{0}$ (1)
    \item $v_3>v_2>v_1\geq{v_4}\geq{0}$ (7.2)
    \item $v_3>v_2\geq{v_4}>v_1\geq{0}$ (6.3)
    \item $v_3\geq{v_4}>v_1\geq{v_2}\geq{0}$

    $v_3\geq{v_4}>v_1+v_2\geq{v_1}\geq{v_2}\geq{0}$ (3.1.7)

    $v_3\geq{v_1+v_2}\geq{v_4}>v_1\geq{v_2}\geq{0}$ (3.2.7)

    $v_1+v_2>v_3\geq{v_4}>v_1\geq{v_2}\geq{0}$ (3.2.5)

    \item $v_3\geq{v_4}>v_2>v_1\geq{0}$

    $v_3\geq{v_4}>v_1+v_2\geq{v_2}>v_1\geq{0}$ (3.1.6)

    $v_3\geq{v_1+v_2}\geq{v_4>}v_2>v_1\geq{0}$ (3.2.6)

    $v_1+v_2\geq{v_3}\geq{v_4}>v_2>v_2\geq{0}$ (3.2.4)

    \item $v_4>v_1\geq{v_2}\geq{v_3}\geq{0}$

    $v_4>v_2+v_3\geq{v_1}\geq{v_2}\geq{v_3}\geq{0}$ (4.1.2)

    $v_2+v_3\geq{v_4}>v_1\geq{v_2}\geq{v_3}\geq{0}$ (4.2.1)
    
    $v_4>v_1\geq{v_2+v_3}\geq{v_2}\geq{v_3}\geq{0}$ (4.1.4)

    \item $v_4>v_1\geq{v_3}>v_2\geq{0}$

    $v_4>v_2+v_3\geq{v_1}\geq{v_3}>v_2\geq{0}$ (4.1.1)

    $v_2+v_3>v_4>v_1\geq{v_3}>v_2\geq{0}$ (4.2.2)

    $v_4>v_1\geq{v_2+v_3}\geq{v_3}>v_2\geq{0}$ (4.1.5)

    \item $v_4>v_2>v_1\geq{v_3}\geq{0}$

    $v_4>v_2+v_3\geq{v_2}>v_1\geq{v_3}\geq{0}$ (4.1.3)

    $v_2+v_3\geq{v_4}>v_2>v_1\geq{v_3}\geq{0}$ (4.2.3)

    \item $v_4>v_2\geq{v_3}>v_1\geq{0}$

    $v_4>{v_1+v_2}\geq{v_2}\geq{v_3}>v_1\geq{0}$ (3.1.2)

    $v_1+v_2\geq{v_4}>v_2\geq{v_3}>v_1\geq{0}$ (3.2.2)

    \item $v_4>v_3>v_1\geq{v_2}\geq{0}$

    $v_4>{v_1+v_2}\geq{v_3}>v_1\geq{v_2}\geq{0}$ (3.1.3)

    $v_1+v_2\geq{v_4}>v_3>v_1\geq{v_2}\geq{0}$ (3.2.3)

    $v_4>v_3>v_1+v_2\geq{v_1}\geq{v_2}\geq{0}$ (3.1.4)

    \item $v_4>v_3>v_2>v_1\geq{0}$

    $v_4>v_1+v_2\geq{v_3}>v_2>v_1\geq{0}$ (3.1.1)

    $v_1+v_2\geq{v_4}>v_3>v_2>v_1\geq{0}$ (3.2.1)

    $v_4>v_3>v_1+v_2\geq{v_2}>v_1\geq{0}$ (3.1.5)    
\end{enumerate}
\end{document}
