
                \documentclass{article}
                \usepackage{graphicx} % Required for inserting images
                \usepackage{xcolor}
                \begin{document}
                
4.2.1
\[1+(A)v_2+(A)v_3+(A)^2v_2v_3\]Substitution no. 1\[v_1\rightarrow{a+2b+c+d}\]\[v_2\rightarrow{a+b+c+d}\]\[v_3\rightarrow{b+c+d}\]\[v_4\rightarrow{a+2b+2c+d}\]\[1+(A)a+2(A)b+2(A)c+2(A)d+(A)^2ab+(A)^2b^{2}+2(A)^2cb+2(A)^2db+(A)^2ac+(A)^2c^{2}+2(A)^2dc+(A)^2ad+(A)^2d^{2}\]All series and their sums\[\sum_{a\geq{0}}(x_1)^{a}\sum_{b\geq{0}}(x_6)^{b}\sum_{c\geq{1}}(x_4)^{c}\sum_{d\geq{0}}(x_0)^{d}=\frac{(x_4)}{(1-x_1)(1-x_6)(1-x_4)(1-x_0)}\]\[(A)\sum_{a\geq{0}}\textcolor{red}{a}(x_1)^{a}\sum_{b\geq{0}}(x_6)^{b}\sum_{c\geq{1}}(x_4)^{c}\sum_{d\geq{0}}(x_0)^{d}=\frac{(A)(x_1)(x_4)}{(1-x_1)^{\textcolor{red}{2}}(1-x_6)(1-x_4)(1-x_0)}\]\[2(A)\sum_{a\geq{0}}(x_1)^{a}\sum_{b\geq{0}}\textcolor{red}{b}(x_6)^{b}\sum_{c\geq{1}}(x_4)^{c}\sum_{d\geq{0}}(x_0)^{d}=\frac{2(A)(x_6)(x_4)}{(1-x_1)(1-x_6)^{\textcolor{red}{2}}(1-x_4)(1-x_0)}\]\[2(A)\sum_{a\geq{0}}(x_1)^{a}\sum_{b\geq{0}}(x_6)^{b}\sum_{c\geq{1}}\textcolor{red}{c}(x_4)^{c}\sum_{d\geq{0}}(x_0)^{d}=\frac{2(A)(x_4)}{(1-x_1)(1-x_6)(1-x_4)^{\textcolor{red}{2}}(1-x_0)}\]\[2(A)\sum_{a\geq{0}}(x_1)^{a}\sum_{b\geq{0}}(x_6)^{b}\sum_{c\geq{1}}(x_4)^{c}\sum_{d\geq{0}}\textcolor{red}{d}(x_0)^{d}=\frac{2(A)(x_4)(x_0)}{(1-x_1)(1-x_6)(1-x_4)(1-x_0)^{\textcolor{red}{2}}}\]\[(A)^{2}\sum_{a\geq{0}}\textcolor{red}{a}(x_1)^{a}\sum_{b\geq{0}}\textcolor{red}{b}(x_6)^{b}\sum_{c\geq{1}}(x_4)^{c}\sum_{d\geq{0}}(x_0)^{d}=\frac{(A^{2})(x_1)(x_6)(x_4)}{(1-x_1)^{\textcolor{red}{2}}(1-x_6)^{\textcolor{red}{2}}(1-x_4)(1-x_0)}\]\[(A)^{2}\sum_{a\geq{0}}(x_1)^{a}\sum_{b\geq{0}}\textcolor{red}{b^{2}}(x_6)^{b}\sum_{c\geq{1}}(x_4)^{c}\sum_{d\geq{0}}(x_0)^{d}=\frac{(A^{2})(x^{2}+x_6)(x_4)}{(1-x_1)(1-x_6)^{\textcolor{red}{3}}(1-x_4)(1-x_0)}\]\[2(A)^{2}\sum_{a\geq{0}}(x_1)^{a}\sum_{b\geq{0}}\textcolor{red}{b}(x_6)^{b}\sum_{c\geq{1}}\textcolor{red}{c}(x_4)^{c}\sum_{d\geq{0}}(x_0)^{d}=\frac{2(A^{2})(x_6)(x_4)}{(1-x_1)(1-x_6)^{\textcolor{red}{2}}(1-x_4)^{\textcolor{red}{2}}(1-x_0)}\]\[2(A)^{2}\sum_{a\geq{0}}(x_1)^{a}\sum_{b\geq{0}}\textcolor{red}{b}(x_6)^{b}\sum_{c\geq{1}}(x_4)^{c}\sum_{d\geq{0}}\textcolor{red}{d}(x_0)^{d}=\frac{2(A^{2})(x_6)(x_4)(x_0)}{(1-x_1)(1-x_6)^{\textcolor{red}{2}}(1-x_4)(1-x_0)^{\textcolor{red}{2}}}\]\[(A)^{2}\sum_{a\geq{0}}\textcolor{red}{a}(x_1)^{a}\sum_{b\geq{0}}(x_6)^{b}\sum_{c\geq{1}}\textcolor{red}{c}(x_4)^{c}\sum_{d\geq{0}}(x_0)^{d}=\frac{(A^{2})(x_1)(x_4)}{(1-x_1)^{\textcolor{red}{2}}(1-x_6)(1-x_4)^{\textcolor{red}{2}}(1-x_0)}\]\[(A)^{2}\sum_{a\geq{0}}(x_1)^{a}\sum_{b\geq{0}}(x_6)^{b}\sum_{c\geq{1}}\textcolor{red}{c^{2}}(x_4)^{c}\sum_{d\geq{0}}(x_0)^{d}=\frac{(A^{2})(x^{2}+x_4)}{(1-x_1)(1-x_6)(1-x_4)^{\textcolor{red}{3}}(1-x_0)}\]\[2(A)^{2}\sum_{a\geq{0}}(x_1)^{a}\sum_{b\geq{0}}(x_6)^{b}\sum_{c\geq{1}}\textcolor{red}{c}(x_4)^{c}\sum_{d\geq{0}}\textcolor{red}{d}(x_0)^{d}=\frac{2(A^{2})(x_4)(x_0)}{(1-x_1)(1-x_6)(1-x_4)^{\textcolor{red}{2}}(1-x_0)^{\textcolor{red}{2}}}\]\[(A)^{2}\sum_{a\geq{0}}\textcolor{red}{a}(x_1)^{a}\sum_{b\geq{0}}(x_6)^{b}\sum_{c\geq{1}}(x_4)^{c}\sum_{d\geq{0}}\textcolor{red}{d}(x_0)^{d}=\frac{(A^{2})(x_1)(x_4)(x_0)}{(1-x_1)^{\textcolor{red}{2}}(1-x_6)(1-x_4)(1-x_0)^{\textcolor{red}{2}}}\]\[(A)^{2}\sum_{a\geq{0}}(x_1)^{a}\sum_{b\geq{0}}(x_6)^{b}\sum_{c\geq{1}}(x_4)^{c}\sum_{d\geq{0}}\textcolor{red}{d^{2}}(x_0)^{d}=\frac{(A^{2})(x_4)(x^{2}+x_0)}{(1-x_1)(1-x_6)(1-x_4)(1-x_0)^{\textcolor{red}{3}}}\]
Total sum
\[+\frac{(x_4)(1-x_1)(1-x_6)^{\textcolor{red}{2}}(1-x_4)^{\textcolor{red}{2}}(1-x_0)^{\textcolor{red}{2}}}{(1-x_1)^{\textcolor{red}{2}}(1-x_6)^{\textcolor{red}{3}}(1-x_4)^{\textcolor{red}{3}}(1-x_0)^{\textcolor{red}{3}}}\]\[+\frac{(A)(x_1)(x_4)(1-x_6)^{\textcolor{red}{2}}(1-x_4)^{\textcolor{red}{2}}(1-x_0)^{\textcolor{red}{2}}}{(1-x_1)^{\textcolor{red}{2}}(1-x_6)^{\textcolor{red}{3}}(1-x_4)^{\textcolor{red}{3}}(1-x_0)^{\textcolor{red}{3}}}\]\[+\frac{2(A)(x_6)(x_4)(1-x_1)(1-x_4)^{\textcolor{red}{2}}(1-x_0)^{\textcolor{red}{2}}(1-x_6)}{(1-x_1)^{\textcolor{red}{2}}(1-x_6)^{\textcolor{red}{3}}(1-x_4)^{\textcolor{red}{3}}(1-x_0)^{\textcolor{red}{3}}}\]\[+\frac{2(A)(x_4)(1-x_1)(1-x_6)^{\textcolor{red}{2}}(1-x_0)^{\textcolor{red}{2}}(1-x_4)}{(1-x_1)^{\textcolor{red}{2}}(1-x_6)^{\textcolor{red}{3}}(1-x_4)^{\textcolor{red}{3}}(1-x_0)^{\textcolor{red}{3}}}\]\[+\frac{2(A)(x_4)(x_0)(1-x_1)(1-x_6)^{\textcolor{red}{2}}(1-x_4)^{\textcolor{red}{2}}(1-x_0)}{(1-x_1)^{\textcolor{red}{2}}(1-x_6)^{\textcolor{red}{3}}(1-x_4)^{\textcolor{red}{3}}(1-x_0)^{\textcolor{red}{3}}}\]\[+\frac{(A)^{2}(x_1)(x_6)(x_4)(1-x_4)^{\textcolor{red}{2}}(1-x_0)^{\textcolor{red}{2}}(1-x_6)}{(1-x_1)^{\textcolor{red}{2}}(1-x_6)^{\textcolor{red}{3}}(1-x_4)^{\textcolor{red}{3}}(1-x_0)^{\textcolor{red}{3}}}\]\[+\frac{(A)^{2}(x^{2}+x_6)(x_4)(1-x_1)(1-x_4)^{\textcolor{red}{2}}(1-x_0)^{\textcolor{red}{2}}}{(1-x_1)^{\textcolor{red}{2}}(1-x_6)^{\textcolor{red}{3}}(1-x_4)^{\textcolor{red}{3}}(1-x_0)^{\textcolor{red}{3}}}\]\[+\frac{2(A)^{2}(x_6)(x_4)(1-x_1)(1-x_6)(1-x_0)^{\textcolor{red}{2}}(1-x_4)}{(1-x_1)^{\textcolor{red}{2}}(1-x_6)^{\textcolor{red}{3}}(1-x_4)^{\textcolor{red}{3}}(1-x_0)^{\textcolor{red}{3}}}\]\[+\frac{2(A)^{2}(x_6)(x_4)(x_0)(1-x_1)(1-x_6)(1-x_4)^{\textcolor{red}{2}}(1-x_0)}{(1-x_1)^{\textcolor{red}{2}}(1-x_6)^{\textcolor{red}{3}}(1-x_4)^{\textcolor{red}{3}}(1-x_0)^{\textcolor{red}{3}}}\]\[+\frac{(A)^{2}(x_1)(x_4)(1-x_6)^{\textcolor{red}{2}}(1-x_0)^{\textcolor{red}{2}}(1-x_4)}{(1-x_1)^{\textcolor{red}{2}}(1-x_6)^{\textcolor{red}{3}}(1-x_4)^{\textcolor{red}{3}}(1-x_0)^{\textcolor{red}{3}}}\]\[+\frac{(A)^{2}(x^{2}+x_4)(1-x_1)(1-x_6)^{\textcolor{red}{2}}(1-x_0)^{\textcolor{red}{2}}}{(1-x_1)^{\textcolor{red}{2}}(1-x_6)^{\textcolor{red}{3}}(1-x_4)^{\textcolor{red}{3}}(1-x_0)^{\textcolor{red}{3}}}\]\[+\frac{2(A)^{2}(x_4)(x_0)(1-x_1)(1-x_6)^{\textcolor{red}{2}}(1-x_4)(1-x_0)}{(1-x_1)^{\textcolor{red}{2}}(1-x_6)^{\textcolor{red}{3}}(1-x_4)^{\textcolor{red}{3}}(1-x_0)^{\textcolor{red}{3}}}\]\[+\frac{(A)^{2}(x_1)(x_4)(x_0)(1-x_6)^{\textcolor{red}{2}}(1-x_4)^{\textcolor{red}{2}}(1-x_0)}{(1-x_1)^{\textcolor{red}{2}}(1-x_6)^{\textcolor{red}{3}}(1-x_4)^{\textcolor{red}{3}}(1-x_0)^{\textcolor{red}{3}}}\]\[+\frac{(A)^{2}(x_4)(x^{2}+x_0)(1-x_1)(1-x_6)^{\textcolor{red}{2}}(1-x_4)^{\textcolor{red}{2}}}{(1-x_1)^{\textcolor{red}{2}}(1-x_6)^{\textcolor{red}{3}}(1-x_4)^{\textcolor{red}{3}}(1-x_0)^{\textcolor{red}{3}}}\]
4.2.2
\[1+(A)v_2+(A)v_3+(A)^2v_2v_3\]Substitution no. 2\[v_1\rightarrow{a+2b+c+d}\]\[v_2\rightarrow{b+c+d}\]\[v_3\rightarrow{a+b+b+c}\]\[v_4\rightarrow{a+2b+2c+d}\]\[1+3(A)b+2(A)c+(A)d+(A)a+(A)^2ba+(A)^2ca+(A)^2da+2(A)^2b^{2}+3(A)^2cb+2(A)^2db+(A)^2c^{2}+(A)^2dc\]All series and their sums\[\sum_{a\geq{1}}(x_1)^{a}\sum_{b\geq{0}}(x_11)^{b}\sum_{c\geq{1}}(x_4)^{c}\sum_{d\geq{0}}(x_1)^{d}=\frac{(x_1)(x_4)}{(1-x_1)^{\textcolor{red}{2}}(1-x_11)(1-x_4)}\]\[3(A)\sum_{a\geq{1}}(x_1)^{a}\sum_{b\geq{0}}\textcolor{red}{b}(x_11)^{b}\sum_{c\geq{1}}(x_4)^{c}\sum_{d\geq{0}}(x_1)^{d}=\frac{3(A)(x_1)(x_11)(x_4)}{(1-x_1)^{\textcolor{red}{2}}(1-x_11)^{\textcolor{red}{2}}(1-x_4)}\]\[2(A)\sum_{a\geq{1}}(x_1)^{a}\sum_{b\geq{0}}(x_11)^{b}\sum_{c\geq{1}}\textcolor{red}{c}(x_4)^{c}\sum_{d\geq{0}}(x_1)^{d}=\frac{2(A)(x_1)(x_4)}{(1-x_1)^{\textcolor{red}{2}}(1-x_11)(1-x_4)^{\textcolor{red}{2}}}\]\[(A)\sum_{a\geq{1}}(x_1)^{a}\sum_{b\geq{0}}(x_11)^{b}\sum_{c\geq{1}}(x_4)^{c}\sum_{d\geq{0}}\textcolor{red}{d}(x_1)^{d}=\frac{(A)(x_1)^{\textcolor{red}{2}}(x_4)}{(1-x_1)^{\textcolor{red}{3}}(1-x_11)(1-x_4)}\]\[(A)\sum_{a\geq{1}}\textcolor{red}{a}(x_1)^{a}\sum_{b\geq{0}}(x_11)^{b}\sum_{c\geq{1}}(x_4)^{c}\sum_{d\geq{0}}(x_1)^{d}=\frac{(A)(x_1)(x_4)}{(1-x_1)^{\textcolor{red}{3}}(1-x_11)(1-x_4)}\]\[(A)^{2}\sum_{a\geq{1}}\textcolor{red}{a}(x_1)^{a}\sum_{b\geq{0}}\textcolor{red}{b}(x_11)^{b}\sum_{c\geq{1}}(x_4)^{c}\sum_{d\geq{0}}(x_1)^{d}=\frac{(A^{2})(x_1)(x_11)(x_4)}{(1-x_1)^{\textcolor{red}{3}}(1-x_11)^{\textcolor{red}{2}}(1-x_4)}\]\[(A)^{2}\sum_{a\geq{1}}\textcolor{red}{a}(x_1)^{a}\sum_{b\geq{0}}(x_11)^{b}\sum_{c\geq{1}}\textcolor{red}{c}(x_4)^{c}\sum_{d\geq{0}}(x_1)^{d}=\frac{(A^{2})(x_1)(x_4)}{(1-x_1)^{\textcolor{red}{3}}(1-x_11)(1-x_4)^{\textcolor{red}{2}}}\]\[(A)^{2}\sum_{a\geq{1}}\textcolor{red}{a}(x_1)^{a}\sum_{b\geq{0}}(x_11)^{b}\sum_{c\geq{1}}(x_4)^{c}\sum_{d\geq{0}}\textcolor{red}{d}(x_1)^{d}=\frac{(A^{2})(x_1)^{\textcolor{red}{2}}(x_4)}{(1-x_1)^{\textcolor{red}{4}}(1-x_11)(1-x_4)}\]\[2(A)^{2}\sum_{a\geq{1}}(x_1)^{a}\sum_{b\geq{0}}\textcolor{red}{b^{2}}(x_11)^{b}\sum_{c\geq{1}}(x_4)^{c}\sum_{d\geq{0}}(x_1)^{d}=\frac{2(A^{2})(x_1)(x^{2}+x_11)(x_4)}{(1-x_1)^{\textcolor{red}{2}}(1-x_11)^{\textcolor{red}{3}}(1-x_4)}\]\[3(A)^{2}\sum_{a\geq{1}}(x_1)^{a}\sum_{b\geq{0}}\textcolor{red}{b}(x_11)^{b}\sum_{c\geq{1}}\textcolor{red}{c}(x_4)^{c}\sum_{d\geq{0}}(x_1)^{d}=\frac{3(A^{2})(x_1)(x_11)(x_4)}{(1-x_1)^{\textcolor{red}{2}}(1-x_11)^{\textcolor{red}{2}}(1-x_4)^{\textcolor{red}{2}}}\]\[2(A)^{2}\sum_{a\geq{1}}(x_1)^{a}\sum_{b\geq{0}}\textcolor{red}{b}(x_11)^{b}\sum_{c\geq{1}}(x_4)^{c}\sum_{d\geq{0}}\textcolor{red}{d}(x_1)^{d}=\frac{2(A^{2})(x_1)^{\textcolor{red}{2}}(x_11)(x_4)}{(1-x_1)^{\textcolor{red}{3}}(1-x_11)^{\textcolor{red}{2}}(1-x_4)}\]\[(A)^{2}\sum_{a\geq{1}}(x_1)^{a}\sum_{b\geq{0}}(x_11)^{b}\sum_{c\geq{1}}\textcolor{red}{c^{2}}(x_4)^{c}\sum_{d\geq{0}}(x_1)^{d}=\frac{(A^{2})(x_1)(x^{2}+x_4)}{(1-x_1)^{\textcolor{red}{2}}(1-x_11)(1-x_4)^{\textcolor{red}{3}}}\]\[(A)^{2}\sum_{a\geq{1}}(x_1)^{a}\sum_{b\geq{0}}(x_11)^{b}\sum_{c\geq{1}}\textcolor{red}{c}(x_4)^{c}\sum_{d\geq{0}}\textcolor{red}{d}(x_1)^{d}=\frac{(A^{2})(x_1)^{\textcolor{red}{2}}(x_4)}{(1-x_1)^{\textcolor{red}{3}}(1-x_11)(1-x_4)^{\textcolor{red}{2}}}\]
Total sum
\[+\frac{(x_1)(x_4)(1-x_11)^{\textcolor{red}{2}}(1-x_4)^{\textcolor{red}{2}}(1-x_1)^{\textcolor{red}{2}}}{(1-x_1)^{\textcolor{red}{4}}(1-x_11)^{\textcolor{red}{3}}(1-x_4)^{\textcolor{red}{3}}}\]\[+\frac{3(A)(x_1)(x_11)(x_4)(1-x_4)^{\textcolor{red}{2}}(1-x_1)^{\textcolor{red}{2}}(1-x_11)}{(1-x_1)^{\textcolor{red}{4}}(1-x_11)^{\textcolor{red}{3}}(1-x_4)^{\textcolor{red}{3}}}\]\[+\frac{2(A)(x_1)(x_4)(1-x_11)^{\textcolor{red}{2}}(1-x_1)^{\textcolor{red}{2}}(1-x_4)}{(1-x_1)^{\textcolor{red}{4}}(1-x_11)^{\textcolor{red}{3}}(1-x_4)^{\textcolor{red}{3}}}\]\[+\frac{(A)(x_1)^{\textcolor{red}{2}}(x_4)(1-x_11)^{\textcolor{red}{2}}(1-x_4)^{\textcolor{red}{2}}(1-x_1)}{(1-x_1)^{\textcolor{red}{4}}(1-x_11)^{\textcolor{red}{3}}(1-x_4)^{\textcolor{red}{3}}}\]\[+\frac{(A)(x_1)(x_4)(1-x_11)^{\textcolor{red}{2}}(1-x_4)^{\textcolor{red}{2}}(1-x_1)}{(1-x_1)^{\textcolor{red}{4}}(1-x_11)^{\textcolor{red}{3}}(1-x_4)^{\textcolor{red}{3}}}\]\[+\frac{(A)^{2}(x_1)(x_11)(x_4)(1-x_4)^{\textcolor{red}{2}}(1-x_1)(1-x_11)}{(1-x_1)^{\textcolor{red}{4}}(1-x_11)^{\textcolor{red}{3}}(1-x_4)^{\textcolor{red}{3}}}\]\[+\frac{(A)^{2}(x_1)(x_4)(1-x_11)^{\textcolor{red}{2}}(1-x_1)(1-x_4)}{(1-x_1)^{\textcolor{red}{4}}(1-x_11)^{\textcolor{red}{3}}(1-x_4)^{\textcolor{red}{3}}}\]\[+\frac{(A)^{2}(x_1)^{\textcolor{red}{2}}(x_4)(1-x_11)^{\textcolor{red}{2}}(1-x_4)^{\textcolor{red}{2}}}{(1-x_1)^{\textcolor{red}{4}}(1-x_11)^{\textcolor{red}{3}}(1-x_4)^{\textcolor{red}{3}}}\]\[+\frac{2(A)^{2}(x_1)(x^{2}+x_11)(x_4)(1-x_1)^{\textcolor{red}{2}}(1-x_4)^{\textcolor{red}{2}}}{(1-x_1)^{\textcolor{red}{4}}(1-x_11)^{\textcolor{red}{3}}(1-x_4)^{\textcolor{red}{3}}}\]\[+\frac{3(A)^{2}(x_1)(x_11)(x_4)(1-x_1)^{\textcolor{red}{2}}(1-x_11)(1-x_4)}{(1-x_1)^{\textcolor{red}{4}}(1-x_11)^{\textcolor{red}{3}}(1-x_4)^{\textcolor{red}{3}}}\]\[+\frac{2(A)^{2}(x_1)^{\textcolor{red}{2}}(x_11)(x_4)(1-x_1)(1-x_11)(1-x_4)^{\textcolor{red}{2}}}{(1-x_1)^{\textcolor{red}{4}}(1-x_11)^{\textcolor{red}{3}}(1-x_4)^{\textcolor{red}{3}}}\]\[+\frac{(A)^{2}(x_1)(x^{2}+x_4)(1-x_1)^{\textcolor{red}{2}}(1-x_11)^{\textcolor{red}{2}}}{(1-x_1)^{\textcolor{red}{4}}(1-x_11)^{\textcolor{red}{3}}(1-x_4)^{\textcolor{red}{3}}}\]\[+\frac{(A)^{2}(x_1)^{\textcolor{red}{2}}(x_4)(1-x_1)(1-x_11)^{\textcolor{red}{2}}(1-x_4)}{(1-x_1)^{\textcolor{red}{4}}(1-x_11)^{\textcolor{red}{3}}(1-x_4)^{\textcolor{red}{3}}}\]
4.2.3
\[1+(A)v_2+(A)v_3+(A)^2v_2v_3\]Substitution no. 3\[v_1\rightarrow{a+c+d}\]\[v_2\rightarrow{a+b+c+d}\]\[v_3\rightarrow{c+d}\]\[v_4\rightarrow{a+b+2c+d}\]\[1+(A)a+(A)b+2(A)c+2(A)d+(A)^2ac+(A)^2bc+(A)^2c^{2}+2(A)^2dc+(A)^2ad+(A)^2bd+(A)^2d^{2}\]All series and their sums\[\sum_{a\geq{0}}(x_1)^{a}\sum_{c\geq{0}}(x_4)^{c}\sum_{d\geq{0}}(x_0)^{d}\sum_{b\geq{1}}(x_2)^{b}=\frac{(x_2)}{(1-x_1)(1-x_4)(1-x_0)(1-x_2)}\]\[(A)\sum_{a\geq{0}}\textcolor{red}{a}(x_1)^{a}\sum_{c\geq{0}}(x_4)^{c}\sum_{d\geq{0}}(x_0)^{d}\sum_{b\geq{1}}(x_2)^{b}=\frac{(A)(x_1)(x_2)}{(1-x_1)^{\textcolor{red}{2}}(1-x_4)(1-x_0)(1-x_2)}\]\[(A)\sum_{a\geq{0}}(x_1)^{a}\sum_{c\geq{0}}(x_4)^{c}\sum_{d\geq{0}}(x_0)^{d}\sum_{b\geq{1}}\textcolor{red}{b}(x_2)^{b}=\frac{(A)(x_2)}{(1-x_1)(1-x_4)(1-x_0)(1-x_2)^{\textcolor{red}{2}}}\]\[2(A)\sum_{a\geq{0}}(x_1)^{a}\sum_{c\geq{0}}\textcolor{red}{c}(x_4)^{c}\sum_{d\geq{0}}(x_0)^{d}\sum_{b\geq{1}}(x_2)^{b}=\frac{2(A)(x_4)(x_2)}{(1-x_1)(1-x_4)^{\textcolor{red}{2}}(1-x_0)(1-x_2)}\]\[2(A)\sum_{a\geq{0}}(x_1)^{a}\sum_{c\geq{0}}(x_4)^{c}\sum_{d\geq{0}}\textcolor{red}{d}(x_0)^{d}\sum_{b\geq{1}}(x_2)^{b}=\frac{2(A)(x_0)(x_2)}{(1-x_1)(1-x_4)(1-x_0)^{\textcolor{red}{2}}(1-x_2)}\]\[(A)^{2}\sum_{a\geq{0}}\textcolor{red}{a}(x_1)^{a}\sum_{c\geq{0}}\textcolor{red}{c}(x_4)^{c}\sum_{d\geq{0}}(x_0)^{d}\sum_{b\geq{1}}(x_2)^{b}=\frac{(A^{2})(x_1)(x_4)(x_2)}{(1-x_1)^{\textcolor{red}{2}}(1-x_4)^{\textcolor{red}{2}}(1-x_0)(1-x_2)}\]\[(A)^{2}\sum_{a\geq{0}}(x_1)^{a}\sum_{c\geq{0}}\textcolor{red}{c}(x_4)^{c}\sum_{d\geq{0}}(x_0)^{d}\sum_{b\geq{1}}\textcolor{red}{b}(x_2)^{b}=\frac{(A^{2})(x_4)(x_2)}{(1-x_1)(1-x_4)^{\textcolor{red}{2}}(1-x_0)(1-x_2)^{\textcolor{red}{2}}}\]\[(A)^{2}\sum_{a\geq{0}}(x_1)^{a}\sum_{c\geq{0}}\textcolor{red}{c^{2}}(x_4)^{c}\sum_{d\geq{0}}(x_0)^{d}\sum_{b\geq{1}}(x_2)^{b}=\frac{(A^{2})(x^{2}+x_4)(x_2)}{(1-x_1)(1-x_4)^{\textcolor{red}{3}}(1-x_0)(1-x_2)}\]\[2(A)^{2}\sum_{a\geq{0}}(x_1)^{a}\sum_{c\geq{0}}\textcolor{red}{c}(x_4)^{c}\sum_{d\geq{0}}\textcolor{red}{d}(x_0)^{d}\sum_{b\geq{1}}(x_2)^{b}=\frac{2(A^{2})(x_4)(x_0)(x_2)}{(1-x_1)(1-x_4)^{\textcolor{red}{2}}(1-x_0)^{\textcolor{red}{2}}(1-x_2)}\]\[(A)^{2}\sum_{a\geq{0}}\textcolor{red}{a}(x_1)^{a}\sum_{c\geq{0}}(x_4)^{c}\sum_{d\geq{0}}\textcolor{red}{d}(x_0)^{d}\sum_{b\geq{1}}(x_2)^{b}=\frac{(A^{2})(x_1)(x_0)(x_2)}{(1-x_1)^{\textcolor{red}{2}}(1-x_4)(1-x_0)^{\textcolor{red}{2}}(1-x_2)}\]\[(A)^{2}\sum_{a\geq{0}}(x_1)^{a}\sum_{c\geq{0}}(x_4)^{c}\sum_{d\geq{0}}\textcolor{red}{d}(x_0)^{d}\sum_{b\geq{1}}\textcolor{red}{b}(x_2)^{b}=\frac{(A^{2})(x_0)(x_2)}{(1-x_1)(1-x_4)(1-x_0)^{\textcolor{red}{2}}(1-x_2)^{\textcolor{red}{2}}}\]\[(A)^{2}\sum_{a\geq{0}}(x_1)^{a}\sum_{c\geq{0}}(x_4)^{c}\sum_{d\geq{0}}\textcolor{red}{d^{2}}(x_0)^{d}\sum_{b\geq{1}}(x_2)^{b}=\frac{(A^{2})(x^{2}+x_0)(x_2)}{(1-x_1)(1-x_4)(1-x_0)^{\textcolor{red}{3}}(1-x_2)}\]
Total sum
\[+\frac{(x_2)(1-x_1)(1-x_2)(1-x_4)^{\textcolor{red}{2}}(1-x_0)^{\textcolor{red}{2}}}{(1-x_1)^{\textcolor{red}{2}}(1-x_4)^{\textcolor{red}{3}}(1-x_0)^{\textcolor{red}{3}}(1-x_2)^{\textcolor{red}{2}}}\]\[+\frac{(A)(x_1)(x_2)(1-x_2)(1-x_4)^{\textcolor{red}{2}}(1-x_0)^{\textcolor{red}{2}}}{(1-x_1)^{\textcolor{red}{2}}(1-x_4)^{\textcolor{red}{3}}(1-x_0)^{\textcolor{red}{3}}(1-x_2)^{\textcolor{red}{2}}}\]\[+\frac{(A)(x_2)(1-x_1)(1-x_4)^{\textcolor{red}{2}}(1-x_0)^{\textcolor{red}{2}}}{(1-x_1)^{\textcolor{red}{2}}(1-x_4)^{\textcolor{red}{3}}(1-x_0)^{\textcolor{red}{3}}(1-x_2)^{\textcolor{red}{2}}}\]\[+\frac{2(A)(x_4)(x_2)(1-x_1)(1-x_2)(1-x_0)^{\textcolor{red}{2}}(1-x_4)}{(1-x_1)^{\textcolor{red}{2}}(1-x_4)^{\textcolor{red}{3}}(1-x_0)^{\textcolor{red}{3}}(1-x_2)^{\textcolor{red}{2}}}\]\[+\frac{2(A)(x_0)(x_2)(1-x_1)(1-x_4)^{\textcolor{red}{2}}(1-x_2)(1-x_0)}{(1-x_1)^{\textcolor{red}{2}}(1-x_4)^{\textcolor{red}{3}}(1-x_0)^{\textcolor{red}{3}}(1-x_2)^{\textcolor{red}{2}}}\]\[+\frac{(A)^{2}(x_1)(x_4)(x_2)(1-x_0)^{\textcolor{red}{2}}(1-x_2)(1-x_4)}{(1-x_1)^{\textcolor{red}{2}}(1-x_4)^{\textcolor{red}{3}}(1-x_0)^{\textcolor{red}{3}}(1-x_2)^{\textcolor{red}{2}}}\]\[+\frac{(A)^{2}(x_4)(x_2)(1-x_1)(1-x_0)^{\textcolor{red}{2}}(1-x_4)}{(1-x_1)^{\textcolor{red}{2}}(1-x_4)^{\textcolor{red}{3}}(1-x_0)^{\textcolor{red}{3}}(1-x_2)^{\textcolor{red}{2}}}\]\[+\frac{(A)^{2}(x^{2}+x_4)(x_2)(1-x_1)(1-x_0)^{\textcolor{red}{2}}(1-x_2)}{(1-x_1)^{\textcolor{red}{2}}(1-x_4)^{\textcolor{red}{3}}(1-x_0)^{\textcolor{red}{3}}(1-x_2)^{\textcolor{red}{2}}}\]\[+\frac{2(A)^{2}(x_4)(x_0)(x_2)(1-x_1)(1-x_4)(1-x_2)(1-x_0)}{(1-x_1)^{\textcolor{red}{2}}(1-x_4)^{\textcolor{red}{3}}(1-x_0)^{\textcolor{red}{3}}(1-x_2)^{\textcolor{red}{2}}}\]\[+\frac{(A)^{2}(x_1)(x_0)(x_2)(1-x_4)^{\textcolor{red}{2}}(1-x_2)(1-x_0)}{(1-x_1)^{\textcolor{red}{2}}(1-x_4)^{\textcolor{red}{3}}(1-x_0)^{\textcolor{red}{3}}(1-x_2)^{\textcolor{red}{2}}}\]\[+\frac{(A)^{2}(x_0)(x_2)(1-x_1)(1-x_4)^{\textcolor{red}{2}}(1-x_0)}{(1-x_1)^{\textcolor{red}{2}}(1-x_4)^{\textcolor{red}{3}}(1-x_0)^{\textcolor{red}{3}}(1-x_2)^{\textcolor{red}{2}}}\]\[+\frac{(A)^{2}(x^{2}+x_0)(x_2)(1-x_1)(1-x_4)^{\textcolor{red}{2}}(1-x_2)}{(1-x_1)^{\textcolor{red}{2}}(1-x_4)^{\textcolor{red}{3}}(1-x_0)^{\textcolor{red}{3}}(1-x_2)^{\textcolor{red}{2}}}\]\[x_0\rightarrow{p^{37}t^{20}}\]\[x_1\rightarrow{p^{26}t^{14}}\]\[x_2\rightarrow{p^{18}t^{10}}\]\[x_3\rightarrow{p^{11}t^{6}}\]\[x_4\rightarrow{p^{44}t^{24}}\]\[x_5\rightarrow{p^{7}t^{4}}\]\[x_6\rightarrow{p^{52}t^{28}}\]\[x_7\rightarrow{p^{15}t^{8}}\]\[x_8\rightarrow{p^{55}t^{30}}\]\[x_9\rightarrow{p^{29}t^{16}}\]\[x_10\rightarrow{p^{48}t^{26}}\]\[x_11\rightarrow{p^{63}t^{34}}\]\end{document}