
                \documentclass{article}
                \usepackage{graphicx} % Required for inserting images
                \usepackage{xcolor}
                \begin{document}
                
6.1
\[1+(A)v_4+(A)v_1+(A)^2v_4v_1-\frac{1}{2}(A)^2v_1^{2}-\frac{1}{2}(A)^2v_1\]Substitution no. 1\[v_1\rightarrow{a}\]\[v_2\rightarrow{a+b+c+d}\]\[v_3\rightarrow{a+b}\]\[v_4\rightarrow{a+b+c}\]\[1+2(A)a+(A)b+(A)c+\frac{1}{2}(A)^2a^{2}+(A)^2ba+(A)^2ca-\frac{1}{2}(A)^2a\]All series and their sums\[\sum_{a\geq{0}}(x_0)^{a}\sum_{b\geq{1}}(x_9)^{b}\sum_{c\geq{1}}(x_2)^{c}\sum_{d\geq{0}}(x_3)^{d}=\frac{(x_9)(x_2)}{(1-x_0)(1-x_9)(1-x_2)(1-x_3)}\]\[2(A)\sum_{a\geq{0}}\textcolor{red}{a}(x_0)^{a}\sum_{b\geq{1}}(x_9)^{b}\sum_{c\geq{1}}(x_2)^{c}\sum_{d\geq{0}}(x_3)^{d}=\frac{2(A)(x_0)(x_9)(x_2)}{(1-x_0)^{\textcolor{red}{2}}(1-x_9)(1-x_2)(1-x_3)}\]\[(A)\sum_{a\geq{0}}(x_0)^{a}\sum_{b\geq{1}}\textcolor{red}{b}(x_9)^{b}\sum_{c\geq{1}}(x_2)^{c}\sum_{d\geq{0}}(x_3)^{d}=\frac{(A)(x_9)(x_2)}{(1-x_0)(1-x_9)^{\textcolor{red}{2}}(1-x_2)(1-x_3)}\]\[(A)\sum_{a\geq{0}}(x_0)^{a}\sum_{b\geq{1}}(x_9)^{b}\sum_{c\geq{1}}\textcolor{red}{c}(x_2)^{c}\sum_{d\geq{0}}(x_3)^{d}=\frac{(A)(x_9)(x_2)}{(1-x_0)(1-x_9)(1-x_2)^{\textcolor{red}{2}}(1-x_3)}\]\[\frac{1}{2}(A)^{2}\sum_{a\geq{0}}\textcolor{red}{a^{2}}(x_0)^{a}\sum_{b\geq{1}}(x_9)^{b}\sum_{c\geq{1}}(x_2)^{c}\sum_{d\geq{0}}(x_3)^{d}=\frac{\frac{1}{2}(A^{2})(x^{2}+x_0)(x_9)(x_2)}{(1-x_0)^{\textcolor{red}{3}}(1-x_9)(1-x_2)(1-x_3)}\]\[(A)^{2}\sum_{a\geq{0}}\textcolor{red}{a}(x_0)^{a}\sum_{b\geq{1}}\textcolor{red}{b}(x_9)^{b}\sum_{c\geq{1}}(x_2)^{c}\sum_{d\geq{0}}(x_3)^{d}=\frac{(A^{2})(x_0)(x_9)(x_2)}{(1-x_0)^{\textcolor{red}{2}}(1-x_9)^{\textcolor{red}{2}}(1-x_2)(1-x_3)}\]\[(A)^{2}\sum_{a\geq{0}}\textcolor{red}{a}(x_0)^{a}\sum_{b\geq{1}}(x_9)^{b}\sum_{c\geq{1}}\textcolor{red}{c}(x_2)^{c}\sum_{d\geq{0}}(x_3)^{d}=\frac{(A^{2})(x_0)(x_9)(x_2)}{(1-x_0)^{\textcolor{red}{2}}(1-x_9)(1-x_2)^{\textcolor{red}{2}}(1-x_3)}\]\[-\frac{1}{2}(A)^{2}\sum_{a\geq{0}}\textcolor{red}{a}(x_0)^{a}\sum_{b\geq{1}}(x_9)^{b}\sum_{c\geq{1}}(x_2)^{c}\sum_{d\geq{0}}(x_3)^{d}=-\frac{\frac{1}{2}(A^{2})(x_0)(x_9)(x_2)}{(1-x_0)^{\textcolor{red}{2}}(1-x_9)(1-x_2)(1-x_3)}\]
Total sum
\[+\frac{(x_9)(x_2)(1-x_0)^{\textcolor{red}{2}}(1-x_9)(1-x_2)}{(1-x_0)^{\textcolor{red}{3}}(1-x_9)^{\textcolor{red}{2}}(1-x_2)^{\textcolor{red}{2}}(1-x_3)}\]\[+\frac{2(A)(x_0)(x_9)(x_2)(1-x_9)(1-x_2)(1-x_0)}{(1-x_0)^{\textcolor{red}{3}}(1-x_9)^{\textcolor{red}{2}}(1-x_2)^{\textcolor{red}{2}}(1-x_3)}\]\[+\frac{(A)(x_9)(x_2)(1-x_0)^{\textcolor{red}{2}}(1-x_2)}{(1-x_0)^{\textcolor{red}{3}}(1-x_9)^{\textcolor{red}{2}}(1-x_2)^{\textcolor{red}{2}}(1-x_3)}\]\[+\frac{(A)(x_9)(x_2)(1-x_0)^{\textcolor{red}{2}}(1-x_9)}{(1-x_0)^{\textcolor{red}{3}}(1-x_9)^{\textcolor{red}{2}}(1-x_2)^{\textcolor{red}{2}}(1-x_3)}\]\[+\frac{\frac{1}{2}(A)^{2}(x^{2}+x_0)(x_9)(x_2)(1-x_9)(1-x_2)}{(1-x_0)^{\textcolor{red}{3}}(1-x_9)^{\textcolor{red}{2}}(1-x_2)^{\textcolor{red}{2}}(1-x_3)}\]\[+\frac{(A)^{2}(x_0)(x_9)(x_2)(1-x_0)(1-x_2)}{(1-x_0)^{\textcolor{red}{3}}(1-x_9)^{\textcolor{red}{2}}(1-x_2)^{\textcolor{red}{2}}(1-x_3)}\]\[+\frac{(A)^{2}(x_0)(x_9)(x_2)(1-x_0)(1-x_9)}{(1-x_0)^{\textcolor{red}{3}}(1-x_9)^{\textcolor{red}{2}}(1-x_2)^{\textcolor{red}{2}}(1-x_3)}\]\[-\frac{\frac{1}{2}(A)^{2}(x_0)(x_9)(x_2)(1-x_0)(1-x_9)(1-x_2)}{(1-x_0)^{\textcolor{red}{3}}(1-x_9)^{\textcolor{red}{2}}(1-x_2)^{\textcolor{red}{2}}(1-x_3)}\]
6.2
\[1+(A)v_4+(A)v_1+(A)^2v_4v_1-\frac{1}{2}(A)^2v_1^{2}-\frac{1}{2}(A)^2v_1\]Substitution no. 2\[v_1\rightarrow{a}\]\[v_2\rightarrow{a+b+c+d}\]\[v_3\rightarrow{a+b+c}\]\[v_4\rightarrow{a+b}\]\[1+2(A)a+(A)b+\frac{1}{2}(A)^2a^{2}+(A)^2ba-\frac{1}{2}(A)^2a\]All series and their sums\[\sum_{a\geq{0}}(x_0)^{a}\sum_{b\geq{1}}(x_9)^{b}\sum_{c\geq{0}}(x_12)^{c}\sum_{d\geq{0}}(x_3)^{d}=\frac{(x_9)}{(1-x_0)(1-x_9)(1-x_12)(1-x_3)}\]\[2(A)\sum_{a\geq{0}}\textcolor{red}{a}(x_0)^{a}\sum_{b\geq{1}}(x_9)^{b}\sum_{c\geq{0}}(x_12)^{c}\sum_{d\geq{0}}(x_3)^{d}=\frac{2(A)(x_0)(x_9)}{(1-x_0)^{\textcolor{red}{2}}(1-x_9)(1-x_12)(1-x_3)}\]\[(A)\sum_{a\geq{0}}(x_0)^{a}\sum_{b\geq{1}}\textcolor{red}{b}(x_9)^{b}\sum_{c\geq{0}}(x_12)^{c}\sum_{d\geq{0}}(x_3)^{d}=\frac{(A)(x_9)}{(1-x_0)(1-x_9)^{\textcolor{red}{2}}(1-x_12)(1-x_3)}\]\[\frac{1}{2}(A)^{2}\sum_{a\geq{0}}\textcolor{red}{a^{2}}(x_0)^{a}\sum_{b\geq{1}}(x_9)^{b}\sum_{c\geq{0}}(x_12)^{c}\sum_{d\geq{0}}(x_3)^{d}=\frac{\frac{1}{2}(A^{2})(x^{2}+x_0)(x_9)}{(1-x_0)^{\textcolor{red}{3}}(1-x_9)(1-x_12)(1-x_3)}\]\[(A)^{2}\sum_{a\geq{0}}\textcolor{red}{a}(x_0)^{a}\sum_{b\geq{1}}\textcolor{red}{b}(x_9)^{b}\sum_{c\geq{0}}(x_12)^{c}\sum_{d\geq{0}}(x_3)^{d}=\frac{(A^{2})(x_0)(x_9)}{(1-x_0)^{\textcolor{red}{2}}(1-x_9)^{\textcolor{red}{2}}(1-x_12)(1-x_3)}\]\[-\frac{1}{2}(A)^{2}\sum_{a\geq{0}}\textcolor{red}{a}(x_0)^{a}\sum_{b\geq{1}}(x_9)^{b}\sum_{c\geq{0}}(x_12)^{c}\sum_{d\geq{0}}(x_3)^{d}=-\frac{\frac{1}{2}(A^{2})(x_0)(x_9)}{(1-x_0)^{\textcolor{red}{2}}(1-x_9)(1-x_12)(1-x_3)}\]
Total sum
\[+\frac{(x_9)(1-x_0)^{\textcolor{red}{2}}(1-x_9)}{(1-x_0)^{\textcolor{red}{3}}(1-x_9)^{\textcolor{red}{2}}(1-x_12)(1-x_3)}\]\[+\frac{2(A)(x_0)(x_9)(1-x_9)(1-x_0)}{(1-x_0)^{\textcolor{red}{3}}(1-x_9)^{\textcolor{red}{2}}(1-x_12)(1-x_3)}\]\[+\frac{(A)(x_9)(1-x_0)^{\textcolor{red}{2}}}{(1-x_0)^{\textcolor{red}{3}}(1-x_9)^{\textcolor{red}{2}}(1-x_12)(1-x_3)}\]\[+\frac{\frac{1}{2}(A)^{2}(x^{2}+x_0)(x_9)(1-x_9)}{(1-x_0)^{\textcolor{red}{3}}(1-x_9)^{\textcolor{red}{2}}(1-x_12)(1-x_3)}\]\[+\frac{(A)^{2}(x_0)(x_9)(1-x_0)}{(1-x_0)^{\textcolor{red}{3}}(1-x_9)^{\textcolor{red}{2}}(1-x_12)(1-x_3)}\]\[-\frac{\frac{1}{2}(A)^{2}(x_0)(x_9)(1-x_0)(1-x_9)}{(1-x_0)^{\textcolor{red}{3}}(1-x_9)^{\textcolor{red}{2}}(1-x_12)(1-x_3)}\]
6.3
\[1+(A)v_4+(A)v_1+(A)^2v_4v_1-\frac{1}{2}(A)^2v_1^{2}-\frac{1}{2}(A)^2v_1\]Substitution no. 3\[v_1\rightarrow{a}\]\[v_2\rightarrow{a+b+c}\]\[v_3\rightarrow{a+b+c+d}\]\[v_4\rightarrow{a+b}\]\[1+2(A)a+(A)b+\frac{1}{2}(A)^2a^{2}+(A)^2ba-\frac{1}{2}(A)^2a\]All series and their sums\[\sum_{a\geq{0}}(x_0)^{a}\sum_{b\geq{1}}(x_9)^{b}\sum_{c\geq{0}}(x_12)^{c}\sum_{d\geq{1}}(x_3)^{d}=\frac{(x_9)(x_3)}{(1-x_0)(1-x_9)(1-x_12)(1-x_3)}\]\[2(A)\sum_{a\geq{0}}\textcolor{red}{a}(x_0)^{a}\sum_{b\geq{1}}(x_9)^{b}\sum_{c\geq{0}}(x_12)^{c}\sum_{d\geq{1}}(x_3)^{d}=\frac{2(A)(x_0)(x_9)(x_3)}{(1-x_0)^{\textcolor{red}{2}}(1-x_9)(1-x_12)(1-x_3)}\]\[(A)\sum_{a\geq{0}}(x_0)^{a}\sum_{b\geq{1}}\textcolor{red}{b}(x_9)^{b}\sum_{c\geq{0}}(x_12)^{c}\sum_{d\geq{1}}(x_3)^{d}=\frac{(A)(x_9)(x_3)}{(1-x_0)(1-x_9)^{\textcolor{red}{2}}(1-x_12)(1-x_3)}\]\[\frac{1}{2}(A)^{2}\sum_{a\geq{0}}\textcolor{red}{a^{2}}(x_0)^{a}\sum_{b\geq{1}}(x_9)^{b}\sum_{c\geq{0}}(x_12)^{c}\sum_{d\geq{1}}(x_3)^{d}=\frac{\frac{1}{2}(A^{2})(x^{2}+x_0)(x_9)(x_3)}{(1-x_0)^{\textcolor{red}{3}}(1-x_9)(1-x_12)(1-x_3)}\]\[(A)^{2}\sum_{a\geq{0}}\textcolor{red}{a}(x_0)^{a}\sum_{b\geq{1}}\textcolor{red}{b}(x_9)^{b}\sum_{c\geq{0}}(x_12)^{c}\sum_{d\geq{1}}(x_3)^{d}=\frac{(A^{2})(x_0)(x_9)(x_3)}{(1-x_0)^{\textcolor{red}{2}}(1-x_9)^{\textcolor{red}{2}}(1-x_12)(1-x_3)}\]\[-\frac{1}{2}(A)^{2}\sum_{a\geq{0}}\textcolor{red}{a}(x_0)^{a}\sum_{b\geq{1}}(x_9)^{b}\sum_{c\geq{0}}(x_12)^{c}\sum_{d\geq{1}}(x_3)^{d}=-\frac{\frac{1}{2}(A^{2})(x_0)(x_9)(x_3)}{(1-x_0)^{\textcolor{red}{2}}(1-x_9)(1-x_12)(1-x_3)}\]
Total sum
\[+\frac{(x_9)(x_3)(1-x_0)^{\textcolor{red}{2}}(1-x_9)}{(1-x_0)^{\textcolor{red}{3}}(1-x_9)^{\textcolor{red}{2}}(1-x_12)(1-x_3)}\]\[+\frac{2(A)(x_0)(x_9)(x_3)(1-x_9)(1-x_0)}{(1-x_0)^{\textcolor{red}{3}}(1-x_9)^{\textcolor{red}{2}}(1-x_12)(1-x_3)}\]\[+\frac{(A)(x_9)(x_3)(1-x_0)^{\textcolor{red}{2}}}{(1-x_0)^{\textcolor{red}{3}}(1-x_9)^{\textcolor{red}{2}}(1-x_12)(1-x_3)}\]\[+\frac{\frac{1}{2}(A)^{2}(x^{2}+x_0)(x_9)(x_3)(1-x_9)}{(1-x_0)^{\textcolor{red}{3}}(1-x_9)^{\textcolor{red}{2}}(1-x_12)(1-x_3)}\]\[+\frac{(A)^{2}(x_0)(x_9)(x_3)(1-x_0)}{(1-x_0)^{\textcolor{red}{3}}(1-x_9)^{\textcolor{red}{2}}(1-x_12)(1-x_3)}\]\[-\frac{\frac{1}{2}(A)^{2}(x_0)(x_9)(x_3)(1-x_0)(1-x_9)}{(1-x_0)^{\textcolor{red}{3}}(1-x_9)^{\textcolor{red}{2}}(1-x_12)(1-x_3)}\]\[x_0\rightarrow{p^{37}t^{20}}\]\[x_1\rightarrow{p^{26}t^{14}}\]\[x_2\rightarrow{p^{18}t^{10}}\]\[x_3\rightarrow{p^{11}t^{6}}\]\[x_4\rightarrow{p^{44}t^{24}}\]\[x_5\rightarrow{p^{7}t^{4}}\]\[x_6\rightarrow{p^{52}t^{28}}\]\[x_7\rightarrow{p^{15}t^{8}}\]\[x_8\rightarrow{p^{55}t^{30}}\]\[x_9\rightarrow{p^{29}t^{16}}\]\[x_10\rightarrow{p^{48}t^{26}}\]\[x_11\rightarrow{p^{63}t^{34}}\]\[x_12\rightarrow{p^{22}t^{12}}\]\end{document}