
                \documentclass{article}
                \usepackage{graphicx} % Required for inserting images
                \usepackage{xcolor}
                \begin{document}
                
8.1.1
\[1+(A)v_4+(A)v_3+(A)^2v_3v_4\]Substitution no. 1\[v_1\rightarrow{2a+b+c+d}\]\[v_2\rightarrow{a+b}\]\[v_3\rightarrow{a+b+c}\]\[v_4\rightarrow{a}\]\[1+2(A)a+(A)b+(A)c+(A)^2a^{2}+(A)^2ba+(A)^2ca\]All series and their sums\[\sum_{a\geq{0}}(x_4)^{a}\sum_{b\geq{0}}(x_9)^{b}\sum_{c\geq{1}}(x_2)^{c}\sum_{d\geq{0}}(x_5)^{d}=\frac{(x_2)}{(1-x_4)(1-x_9)(1-x_2)(1-x_5)}\]\[2(A)\sum_{a\geq{0}}\textcolor{red}{a}(x_4)^{a}\sum_{b\geq{0}}(x_9)^{b}\sum_{c\geq{1}}(x_2)^{c}\sum_{d\geq{0}}(x_5)^{d}=\frac{2(A)(x_4)(x_2)}{(1-x_4)^{\textcolor{red}{2}}(1-x_9)(1-x_2)(1-x_5)}\]\[(A)\sum_{a\geq{0}}(x_4)^{a}\sum_{b\geq{0}}\textcolor{red}{b}(x_9)^{b}\sum_{c\geq{1}}(x_2)^{c}\sum_{d\geq{0}}(x_5)^{d}=\frac{(A)(x_9)(x_2)}{(1-x_4)(1-x_9)^{\textcolor{red}{2}}(1-x_2)(1-x_5)}\]\[(A)\sum_{a\geq{0}}(x_4)^{a}\sum_{b\geq{0}}(x_9)^{b}\sum_{c\geq{1}}\textcolor{red}{c}(x_2)^{c}\sum_{d\geq{0}}(x_5)^{d}=\frac{(A)(x_2)}{(1-x_4)(1-x_9)(1-x_2)^{\textcolor{red}{2}}(1-x_5)}\]\[(A)^{2}\sum_{a\geq{0}}\textcolor{red}{a^{2}}(x_4)^{a}\sum_{b\geq{0}}(x_9)^{b}\sum_{c\geq{1}}(x_2)^{c}\sum_{d\geq{0}}(x_5)^{d}=\frac{(A^{2})(x^{2}+x_4)(x_2)}{(1-x_4)^{\textcolor{red}{3}}(1-x_9)(1-x_2)(1-x_5)}\]\[(A)^{2}\sum_{a\geq{0}}\textcolor{red}{a}(x_4)^{a}\sum_{b\geq{0}}\textcolor{red}{b}(x_9)^{b}\sum_{c\geq{1}}(x_2)^{c}\sum_{d\geq{0}}(x_5)^{d}=\frac{(A^{2})(x_4)(x_9)(x_2)}{(1-x_4)^{\textcolor{red}{2}}(1-x_9)^{\textcolor{red}{2}}(1-x_2)(1-x_5)}\]\[(A)^{2}\sum_{a\geq{0}}\textcolor{red}{a}(x_4)^{a}\sum_{b\geq{0}}(x_9)^{b}\sum_{c\geq{1}}\textcolor{red}{c}(x_2)^{c}\sum_{d\geq{0}}(x_5)^{d}=\frac{(A^{2})(x_4)(x_2)}{(1-x_4)^{\textcolor{red}{2}}(1-x_9)(1-x_2)^{\textcolor{red}{2}}(1-x_5)}\]
Total sum
\[+\frac{(x_2)(1-x_4)^{\textcolor{red}{2}}(1-x_9)(1-x_2)}{(1-x_4)^{\textcolor{red}{3}}(1-x_9)^{\textcolor{red}{2}}(1-x_2)^{\textcolor{red}{2}}(1-x_5)}\]\[+\frac{2(A)(x_4)(x_2)(1-x_9)(1-x_2)(1-x_4)}{(1-x_4)^{\textcolor{red}{3}}(1-x_9)^{\textcolor{red}{2}}(1-x_2)^{\textcolor{red}{2}}(1-x_5)}\]\[+\frac{(A)(x_9)(x_2)(1-x_4)^{\textcolor{red}{2}}(1-x_2)}{(1-x_4)^{\textcolor{red}{3}}(1-x_9)^{\textcolor{red}{2}}(1-x_2)^{\textcolor{red}{2}}(1-x_5)}\]\[+\frac{(A)(x_2)(1-x_4)^{\textcolor{red}{2}}(1-x_9)}{(1-x_4)^{\textcolor{red}{3}}(1-x_9)^{\textcolor{red}{2}}(1-x_2)^{\textcolor{red}{2}}(1-x_5)}\]\[+\frac{(A)^{2}(x^{2}+x_4)(x_2)(1-x_9)(1-x_2)}{(1-x_4)^{\textcolor{red}{3}}(1-x_9)^{\textcolor{red}{2}}(1-x_2)^{\textcolor{red}{2}}(1-x_5)}\]\[+\frac{(A)^{2}(x_4)(x_9)(x_2)(1-x_4)(1-x_2)}{(1-x_4)^{\textcolor{red}{3}}(1-x_9)^{\textcolor{red}{2}}(1-x_2)^{\textcolor{red}{2}}(1-x_5)}\]\[+\frac{(A)^{2}(x_4)(x_2)(1-x_4)(1-x_9)}{(1-x_4)^{\textcolor{red}{3}}(1-x_9)^{\textcolor{red}{2}}(1-x_2)^{\textcolor{red}{2}}(1-x_5)}\]
8.1.2
\[1+(A)v_4+(A)v_3+(A)^2v_3v_4\]Substitution no. 2\[v_1\rightarrow{a+2b+2c+d}\]\[v_2\rightarrow{a+2b+c}\]\[v_3\rightarrow{a+b+c}\]\[v_4\rightarrow{b+c}\]\[1+2(A)b+2(A)c+(A)a+(A)^2ab+(A)^2b^{2}+2(A)^2cb+(A)^2ac+(A)^2c^{2}\]All series and their sums\[\sum_{a\geq{0}}(x_9)^{a}\sum_{b\geq{0}}(x_8)^{b}\sum_{c\geq{0}}(x_4)^{c}\sum_{d\geq{0}}(x_5)^{d}=\frac{1}{(1-x_9)(1-x_8)(1-x_4)(1-x_5)}\]\[2(A)\sum_{a\geq{0}}(x_9)^{a}\sum_{b\geq{0}}\textcolor{red}{b}(x_8)^{b}\sum_{c\geq{0}}(x_4)^{c}\sum_{d\geq{0}}(x_5)^{d}=\frac{2(A)(x_8)}{(1-x_9)(1-x_8)^{\textcolor{red}{2}}(1-x_4)(1-x_5)}\]\[2(A)\sum_{a\geq{0}}(x_9)^{a}\sum_{b\geq{0}}(x_8)^{b}\sum_{c\geq{0}}\textcolor{red}{c}(x_4)^{c}\sum_{d\geq{0}}(x_5)^{d}=\frac{2(A)(x_4)}{(1-x_9)(1-x_8)(1-x_4)^{\textcolor{red}{2}}(1-x_5)}\]\[(A)\sum_{a\geq{0}}\textcolor{red}{a}(x_9)^{a}\sum_{b\geq{0}}(x_8)^{b}\sum_{c\geq{0}}(x_4)^{c}\sum_{d\geq{0}}(x_5)^{d}=\frac{(A)(x_9)}{(1-x_9)^{\textcolor{red}{2}}(1-x_8)(1-x_4)(1-x_5)}\]\[(A)^{2}\sum_{a\geq{0}}\textcolor{red}{a}(x_9)^{a}\sum_{b\geq{0}}\textcolor{red}{b}(x_8)^{b}\sum_{c\geq{0}}(x_4)^{c}\sum_{d\geq{0}}(x_5)^{d}=\frac{(A^{2})(x_9)(x_8)}{(1-x_9)^{\textcolor{red}{2}}(1-x_8)^{\textcolor{red}{2}}(1-x_4)(1-x_5)}\]\[(A)^{2}\sum_{a\geq{0}}(x_9)^{a}\sum_{b\geq{0}}\textcolor{red}{b^{2}}(x_8)^{b}\sum_{c\geq{0}}(x_4)^{c}\sum_{d\geq{0}}(x_5)^{d}=\frac{(A^{2})(x^{2}+x_8)}{(1-x_9)(1-x_8)^{\textcolor{red}{3}}(1-x_4)(1-x_5)}\]\[2(A)^{2}\sum_{a\geq{0}}(x_9)^{a}\sum_{b\geq{0}}\textcolor{red}{b}(x_8)^{b}\sum_{c\geq{0}}\textcolor{red}{c}(x_4)^{c}\sum_{d\geq{0}}(x_5)^{d}=\frac{2(A^{2})(x_8)(x_4)}{(1-x_9)(1-x_8)^{\textcolor{red}{2}}(1-x_4)^{\textcolor{red}{2}}(1-x_5)}\]\[(A)^{2}\sum_{a\geq{0}}\textcolor{red}{a}(x_9)^{a}\sum_{b\geq{0}}(x_8)^{b}\sum_{c\geq{0}}\textcolor{red}{c}(x_4)^{c}\sum_{d\geq{0}}(x_5)^{d}=\frac{(A^{2})(x_9)(x_4)}{(1-x_9)^{\textcolor{red}{2}}(1-x_8)(1-x_4)^{\textcolor{red}{2}}(1-x_5)}\]\[(A)^{2}\sum_{a\geq{0}}(x_9)^{a}\sum_{b\geq{0}}(x_8)^{b}\sum_{c\geq{0}}\textcolor{red}{c^{2}}(x_4)^{c}\sum_{d\geq{0}}(x_5)^{d}=\frac{(A^{2})(x^{2}+x_4)}{(1-x_9)(1-x_8)(1-x_4)^{\textcolor{red}{3}}(1-x_5)}\]
Total sum
\[+\frac{(1-x_8)^{\textcolor{red}{2}}(1-x_4)^{\textcolor{red}{2}}(1-x_9)}{(1-x_9)^{\textcolor{red}{2}}(1-x_8)^{\textcolor{red}{3}}(1-x_4)^{\textcolor{red}{3}}(1-x_5)}\]\[+\frac{2(A)(x_8)(1-x_4)^{\textcolor{red}{2}}(1-x_9)(1-x_8)}{(1-x_9)^{\textcolor{red}{2}}(1-x_8)^{\textcolor{red}{3}}(1-x_4)^{\textcolor{red}{3}}(1-x_5)}\]\[+\frac{2(A)(x_4)(1-x_8)^{\textcolor{red}{2}}(1-x_9)(1-x_4)}{(1-x_9)^{\textcolor{red}{2}}(1-x_8)^{\textcolor{red}{3}}(1-x_4)^{\textcolor{red}{3}}(1-x_5)}\]\[+\frac{(A)(x_9)(1-x_8)^{\textcolor{red}{2}}(1-x_4)^{\textcolor{red}{2}}}{(1-x_9)^{\textcolor{red}{2}}(1-x_8)^{\textcolor{red}{3}}(1-x_4)^{\textcolor{red}{3}}(1-x_5)}\]\[+\frac{(A)^{2}(x_9)(x_8)(1-x_4)^{\textcolor{red}{2}}(1-x_8)}{(1-x_9)^{\textcolor{red}{2}}(1-x_8)^{\textcolor{red}{3}}(1-x_4)^{\textcolor{red}{3}}(1-x_5)}\]\[+\frac{(A)^{2}(x^{2}+x_8)(1-x_9)(1-x_4)^{\textcolor{red}{2}}}{(1-x_9)^{\textcolor{red}{2}}(1-x_8)^{\textcolor{red}{3}}(1-x_4)^{\textcolor{red}{3}}(1-x_5)}\]\[+\frac{2(A)^{2}(x_8)(x_4)(1-x_9)(1-x_8)(1-x_4)}{(1-x_9)^{\textcolor{red}{2}}(1-x_8)^{\textcolor{red}{3}}(1-x_4)^{\textcolor{red}{3}}(1-x_5)}\]\[+\frac{(A)^{2}(x_9)(x_4)(1-x_8)^{\textcolor{red}{2}}(1-x_4)}{(1-x_9)^{\textcolor{red}{2}}(1-x_8)^{\textcolor{red}{3}}(1-x_4)^{\textcolor{red}{3}}(1-x_5)}\]\[+\frac{(A)^{2}(x^{2}+x_4)(1-x_9)(1-x_8)^{\textcolor{red}{2}}}{(1-x_9)^{\textcolor{red}{2}}(1-x_8)^{\textcolor{red}{3}}(1-x_4)^{\textcolor{red}{3}}(1-x_5)}\]
8.1.3
\[1+(A)v_4+(A)v_3+(A)^2v_3v_4\]Substitution no. 3\[v_1\rightarrow{a+2b+2c+d}\]\[v_2\rightarrow{a+2b+c}\]\[v_3\rightarrow{a+b+c}\]\[v_4\rightarrow{b+c}\]\[1+2(A)b+2(A)c+(A)a+(A)^2ab+(A)^2b^{2}+2(A)^2cb+(A)^2ac+(A)^2c^{2}\]All series and their sums\[\sum_{a\geq{1}}(x_9)^{a}\sum_{b\geq{0}}(x_8)^{b}\sum_{c\geq{0}}(x_4)^{c}\sum_{d\geq{0}}(x_5)^{d}=\frac{(x_9)}{(1-x_9)(1-x_8)(1-x_4)(1-x_5)}\]\[2(A)\sum_{a\geq{1}}(x_9)^{a}\sum_{b\geq{0}}\textcolor{red}{b}(x_8)^{b}\sum_{c\geq{0}}(x_4)^{c}\sum_{d\geq{0}}(x_5)^{d}=\frac{2(A)(x_9)(x_8)}{(1-x_9)(1-x_8)^{\textcolor{red}{2}}(1-x_4)(1-x_5)}\]\[2(A)\sum_{a\geq{1}}(x_9)^{a}\sum_{b\geq{0}}(x_8)^{b}\sum_{c\geq{0}}\textcolor{red}{c}(x_4)^{c}\sum_{d\geq{0}}(x_5)^{d}=\frac{2(A)(x_9)(x_4)}{(1-x_9)(1-x_8)(1-x_4)^{\textcolor{red}{2}}(1-x_5)}\]\[(A)\sum_{a\geq{1}}\textcolor{red}{a}(x_9)^{a}\sum_{b\geq{0}}(x_8)^{b}\sum_{c\geq{0}}(x_4)^{c}\sum_{d\geq{0}}(x_5)^{d}=\frac{(A)(x_9)}{(1-x_9)^{\textcolor{red}{2}}(1-x_8)(1-x_4)(1-x_5)}\]\[(A)^{2}\sum_{a\geq{1}}\textcolor{red}{a}(x_9)^{a}\sum_{b\geq{0}}\textcolor{red}{b}(x_8)^{b}\sum_{c\geq{0}}(x_4)^{c}\sum_{d\geq{0}}(x_5)^{d}=\frac{(A^{2})(x_9)(x_8)}{(1-x_9)^{\textcolor{red}{2}}(1-x_8)^{\textcolor{red}{2}}(1-x_4)(1-x_5)}\]\[(A)^{2}\sum_{a\geq{1}}(x_9)^{a}\sum_{b\geq{0}}\textcolor{red}{b^{2}}(x_8)^{b}\sum_{c\geq{0}}(x_4)^{c}\sum_{d\geq{0}}(x_5)^{d}=\frac{(A^{2})(x_9)(x^{2}+x_8)}{(1-x_9)(1-x_8)^{\textcolor{red}{3}}(1-x_4)(1-x_5)}\]\[2(A)^{2}\sum_{a\geq{1}}(x_9)^{a}\sum_{b\geq{0}}\textcolor{red}{b}(x_8)^{b}\sum_{c\geq{0}}\textcolor{red}{c}(x_4)^{c}\sum_{d\geq{0}}(x_5)^{d}=\frac{2(A^{2})(x_9)(x_8)(x_4)}{(1-x_9)(1-x_8)^{\textcolor{red}{2}}(1-x_4)^{\textcolor{red}{2}}(1-x_5)}\]\[(A)^{2}\sum_{a\geq{1}}\textcolor{red}{a}(x_9)^{a}\sum_{b\geq{0}}(x_8)^{b}\sum_{c\geq{0}}\textcolor{red}{c}(x_4)^{c}\sum_{d\geq{0}}(x_5)^{d}=\frac{(A^{2})(x_9)(x_4)}{(1-x_9)^{\textcolor{red}{2}}(1-x_8)(1-x_4)^{\textcolor{red}{2}}(1-x_5)}\]\[(A)^{2}\sum_{a\geq{1}}(x_9)^{a}\sum_{b\geq{0}}(x_8)^{b}\sum_{c\geq{0}}\textcolor{red}{c^{2}}(x_4)^{c}\sum_{d\geq{0}}(x_5)^{d}=\frac{(A^{2})(x_9)(x^{2}+x_4)}{(1-x_9)(1-x_8)(1-x_4)^{\textcolor{red}{3}}(1-x_5)}\]
Total sum
\[+\frac{(x_9)(1-x_8)^{\textcolor{red}{2}}(1-x_4)^{\textcolor{red}{2}}(1-x_9)}{(1-x_9)^{\textcolor{red}{2}}(1-x_8)^{\textcolor{red}{3}}(1-x_4)^{\textcolor{red}{3}}(1-x_5)}\]\[+\frac{2(A)(x_9)(x_8)(1-x_4)^{\textcolor{red}{2}}(1-x_9)(1-x_8)}{(1-x_9)^{\textcolor{red}{2}}(1-x_8)^{\textcolor{red}{3}}(1-x_4)^{\textcolor{red}{3}}(1-x_5)}\]\[+\frac{2(A)(x_9)(x_4)(1-x_8)^{\textcolor{red}{2}}(1-x_9)(1-x_4)}{(1-x_9)^{\textcolor{red}{2}}(1-x_8)^{\textcolor{red}{3}}(1-x_4)^{\textcolor{red}{3}}(1-x_5)}\]\[+\frac{(A)(x_9)(1-x_8)^{\textcolor{red}{2}}(1-x_4)^{\textcolor{red}{2}}}{(1-x_9)^{\textcolor{red}{2}}(1-x_8)^{\textcolor{red}{3}}(1-x_4)^{\textcolor{red}{3}}(1-x_5)}\]\[+\frac{(A)^{2}(x_9)(x_8)(1-x_4)^{\textcolor{red}{2}}(1-x_8)}{(1-x_9)^{\textcolor{red}{2}}(1-x_8)^{\textcolor{red}{3}}(1-x_4)^{\textcolor{red}{3}}(1-x_5)}\]\[+\frac{(A)^{2}(x_9)(x^{2}+x_8)(1-x_9)(1-x_4)^{\textcolor{red}{2}}}{(1-x_9)^{\textcolor{red}{2}}(1-x_8)^{\textcolor{red}{3}}(1-x_4)^{\textcolor{red}{3}}(1-x_5)}\]\[+\frac{2(A)^{2}(x_9)(x_8)(x_4)(1-x_9)(1-x_8)(1-x_4)}{(1-x_9)^{\textcolor{red}{2}}(1-x_8)^{\textcolor{red}{3}}(1-x_4)^{\textcolor{red}{3}}(1-x_5)}\]\[+\frac{(A)^{2}(x_9)(x_4)(1-x_8)^{\textcolor{red}{2}}(1-x_4)}{(1-x_9)^{\textcolor{red}{2}}(1-x_8)^{\textcolor{red}{3}}(1-x_4)^{\textcolor{red}{3}}(1-x_5)}\]\[+\frac{(A)^{2}(x_9)(x^{2}+x_4)(1-x_9)(1-x_8)^{\textcolor{red}{2}}}{(1-x_9)^{\textcolor{red}{2}}(1-x_8)^{\textcolor{red}{3}}(1-x_4)^{\textcolor{red}{3}}(1-x_5)}\]
8.1.4
\[1+(A)v_4+(A)v_3+(A)^2v_3v_4\]Substitution no. 4\[v_1\rightarrow{2a+b+c+d}\]\[v_2\rightarrow{2a+b+c}\]\[v_3\rightarrow{a}\]\[v_4\rightarrow{a+b}\]\[1+2(A)a+(A)b+(A)^2a^{2}+(A)^2ab\]All series and their sums\[\sum_{a\geq{0}}(x_8)^{a}\sum_{b\geq{0}}(x_1)^{b}\sum_{c\geq{1}}(x_2)^{c}\sum_{d\geq{0}}(x_5)^{d}=\frac{(x_2)}{(1-x_8)(1-x_1)(1-x_2)(1-x_5)}\]\[2(A)\sum_{a\geq{0}}\textcolor{red}{a}(x_8)^{a}\sum_{b\geq{0}}(x_1)^{b}\sum_{c\geq{1}}(x_2)^{c}\sum_{d\geq{0}}(x_5)^{d}=\frac{2(A)(x_8)(x_2)}{(1-x_8)^{\textcolor{red}{2}}(1-x_1)(1-x_2)(1-x_5)}\]\[(A)\sum_{a\geq{0}}(x_8)^{a}\sum_{b\geq{0}}\textcolor{red}{b}(x_1)^{b}\sum_{c\geq{1}}(x_2)^{c}\sum_{d\geq{0}}(x_5)^{d}=\frac{(A)(x_1)(x_2)}{(1-x_8)(1-x_1)^{\textcolor{red}{2}}(1-x_2)(1-x_5)}\]\[(A)^{2}\sum_{a\geq{0}}\textcolor{red}{a^{2}}(x_8)^{a}\sum_{b\geq{0}}(x_1)^{b}\sum_{c\geq{1}}(x_2)^{c}\sum_{d\geq{0}}(x_5)^{d}=\frac{(A^{2})(x^{2}+x_8)(x_2)}{(1-x_8)^{\textcolor{red}{3}}(1-x_1)(1-x_2)(1-x_5)}\]\[(A)^{2}\sum_{a\geq{0}}\textcolor{red}{a}(x_8)^{a}\sum_{b\geq{0}}\textcolor{red}{b}(x_1)^{b}\sum_{c\geq{1}}(x_2)^{c}\sum_{d\geq{0}}(x_5)^{d}=\frac{(A^{2})(x_8)(x_1)(x_2)}{(1-x_8)^{\textcolor{red}{2}}(1-x_1)^{\textcolor{red}{2}}(1-x_2)(1-x_5)}\]
Total sum
\[+\frac{(x_2)(1-x_8)^{\textcolor{red}{2}}(1-x_1)}{(1-x_8)^{\textcolor{red}{3}}(1-x_1)^{\textcolor{red}{2}}(1-x_2)(1-x_5)}\]\[+\frac{2(A)(x_8)(x_2)(1-x_1)(1-x_8)}{(1-x_8)^{\textcolor{red}{3}}(1-x_1)^{\textcolor{red}{2}}(1-x_2)(1-x_5)}\]\[+\frac{(A)(x_1)(x_2)(1-x_8)^{\textcolor{red}{2}}}{(1-x_8)^{\textcolor{red}{3}}(1-x_1)^{\textcolor{red}{2}}(1-x_2)(1-x_5)}\]\[+\frac{(A)^{2}(x^{2}+x_8)(x_2)(1-x_1)}{(1-x_8)^{\textcolor{red}{3}}(1-x_1)^{\textcolor{red}{2}}(1-x_2)(1-x_5)}\]\[+\frac{(A)^{2}(x_8)(x_1)(x_2)(1-x_8)}{(1-x_8)^{\textcolor{red}{3}}(1-x_1)^{\textcolor{red}{2}}(1-x_2)(1-x_5)}\]
8.1.5
\[1+(A)v_4+(A)v_3+(A)^2v_3v_4\]Substitution no. 5\[v_1\rightarrow{2a+b+c+d}\]\[v_2\rightarrow{2a+b+c}\]\[v_3\rightarrow{a+b}\]\[v_4\rightarrow{a}\]\[1+2(A)a+(A)b+(A)^2a^{2}+(A)^2ba\]All series and their sums\[\sum_{a\geq{0}}(x_8)^{a}\sum_{b\geq{0}}(x_9)^{b}\sum_{c\geq{1}}(x_2)^{c}\sum_{d\geq{0}}(x_5)^{d}=\frac{(x_2)}{(1-x_8)(1-x_9)(1-x_2)(1-x_5)}\]\[2(A)\sum_{a\geq{0}}\textcolor{red}{a}(x_8)^{a}\sum_{b\geq{0}}(x_9)^{b}\sum_{c\geq{1}}(x_2)^{c}\sum_{d\geq{0}}(x_5)^{d}=\frac{2(A)(x_8)(x_2)}{(1-x_8)^{\textcolor{red}{2}}(1-x_9)(1-x_2)(1-x_5)}\]\[(A)\sum_{a\geq{0}}(x_8)^{a}\sum_{b\geq{0}}\textcolor{red}{b}(x_9)^{b}\sum_{c\geq{1}}(x_2)^{c}\sum_{d\geq{0}}(x_5)^{d}=\frac{(A)(x_9)(x_2)}{(1-x_8)(1-x_9)^{\textcolor{red}{2}}(1-x_2)(1-x_5)}\]\[(A)^{2}\sum_{a\geq{0}}\textcolor{red}{a^{2}}(x_8)^{a}\sum_{b\geq{0}}(x_9)^{b}\sum_{c\geq{1}}(x_2)^{c}\sum_{d\geq{0}}(x_5)^{d}=\frac{(A^{2})(x^{2}+x_8)(x_2)}{(1-x_8)^{\textcolor{red}{3}}(1-x_9)(1-x_2)(1-x_5)}\]\[(A)^{2}\sum_{a\geq{0}}\textcolor{red}{a}(x_8)^{a}\sum_{b\geq{0}}\textcolor{red}{b}(x_9)^{b}\sum_{c\geq{1}}(x_2)^{c}\sum_{d\geq{0}}(x_5)^{d}=\frac{(A^{2})(x_8)(x_9)(x_2)}{(1-x_8)^{\textcolor{red}{2}}(1-x_9)^{\textcolor{red}{2}}(1-x_2)(1-x_5)}\]
Total sum
\[+\frac{(x_2)(1-x_8)^{\textcolor{red}{2}}(1-x_9)}{(1-x_8)^{\textcolor{red}{3}}(1-x_9)^{\textcolor{red}{2}}(1-x_2)(1-x_5)}\]\[+\frac{2(A)(x_8)(x_2)(1-x_9)(1-x_8)}{(1-x_8)^{\textcolor{red}{3}}(1-x_9)^{\textcolor{red}{2}}(1-x_2)(1-x_5)}\]\[+\frac{(A)(x_9)(x_2)(1-x_8)^{\textcolor{red}{2}}}{(1-x_8)^{\textcolor{red}{3}}(1-x_9)^{\textcolor{red}{2}}(1-x_2)(1-x_5)}\]\[+\frac{(A)^{2}(x^{2}+x_8)(x_2)(1-x_9)}{(1-x_8)^{\textcolor{red}{3}}(1-x_9)^{\textcolor{red}{2}}(1-x_2)(1-x_5)}\]\[+\frac{(A)^{2}(x_8)(x_9)(x_2)(1-x_8)}{(1-x_8)^{\textcolor{red}{3}}(1-x_9)^{\textcolor{red}{2}}(1-x_2)(1-x_5)}\]
8.1.6
\[1+(A)v_4+(A)v_3+(A)^2v_3v_4\]Substitution no. 6\[v_1\rightarrow{2a+b+c}\]\[v_2\rightarrow{2a+b+c+d}\]\[v_3\rightarrow{a+b}\]\[v_4\rightarrow{a}\]\[1+2(A)a+(A)b+(A)^2a^{2}+(A)^2ba\]All series and their sums\[\sum_{a\geq{0}}(x_8)^{a}\sum_{b\geq{0}}(x_9)^{b}\sum_{c\geq{0}}(x_2)^{c}\sum_{d\geq{1}}(x_3)^{d}=\frac{(x_3)}{(1-x_8)(1-x_9)(1-x_2)(1-x_3)}\]\[2(A)\sum_{a\geq{0}}\textcolor{red}{a}(x_8)^{a}\sum_{b\geq{0}}(x_9)^{b}\sum_{c\geq{0}}(x_2)^{c}\sum_{d\geq{1}}(x_3)^{d}=\frac{2(A)(x_8)(x_3)}{(1-x_8)^{\textcolor{red}{2}}(1-x_9)(1-x_2)(1-x_3)}\]\[(A)\sum_{a\geq{0}}(x_8)^{a}\sum_{b\geq{0}}\textcolor{red}{b}(x_9)^{b}\sum_{c\geq{0}}(x_2)^{c}\sum_{d\geq{1}}(x_3)^{d}=\frac{(A)(x_9)(x_3)}{(1-x_8)(1-x_9)^{\textcolor{red}{2}}(1-x_2)(1-x_3)}\]\[(A)^{2}\sum_{a\geq{0}}\textcolor{red}{a^{2}}(x_8)^{a}\sum_{b\geq{0}}(x_9)^{b}\sum_{c\geq{0}}(x_2)^{c}\sum_{d\geq{1}}(x_3)^{d}=\frac{(A^{2})(x^{2}+x_8)(x_3)}{(1-x_8)^{\textcolor{red}{3}}(1-x_9)(1-x_2)(1-x_3)}\]\[(A)^{2}\sum_{a\geq{0}}\textcolor{red}{a}(x_8)^{a}\sum_{b\geq{0}}\textcolor{red}{b}(x_9)^{b}\sum_{c\geq{0}}(x_2)^{c}\sum_{d\geq{1}}(x_3)^{d}=\frac{(A^{2})(x_8)(x_9)(x_3)}{(1-x_8)^{\textcolor{red}{2}}(1-x_9)^{\textcolor{red}{2}}(1-x_2)(1-x_3)}\]
Total sum
\[+\frac{(x_3)(1-x_8)^{\textcolor{red}{2}}(1-x_9)}{(1-x_8)^{\textcolor{red}{3}}(1-x_9)^{\textcolor{red}{2}}(1-x_2)(1-x_3)}\]\[+\frac{2(A)(x_8)(x_3)(1-x_9)(1-x_8)}{(1-x_8)^{\textcolor{red}{3}}(1-x_9)^{\textcolor{red}{2}}(1-x_2)(1-x_3)}\]\[+\frac{(A)(x_9)(x_3)(1-x_8)^{\textcolor{red}{2}}}{(1-x_8)^{\textcolor{red}{3}}(1-x_9)^{\textcolor{red}{2}}(1-x_2)(1-x_3)}\]\[+\frac{(A)^{2}(x^{2}+x_8)(x_3)(1-x_9)}{(1-x_8)^{\textcolor{red}{3}}(1-x_9)^{\textcolor{red}{2}}(1-x_2)(1-x_3)}\]\[+\frac{(A)^{2}(x_8)(x_9)(x_3)(1-x_8)}{(1-x_8)^{\textcolor{red}{3}}(1-x_9)^{\textcolor{red}{2}}(1-x_2)(1-x_3)}\]
8.1.7
\[1+(A)v_4+(A)v_3+(A)^2v_3v_4\]Substitution no. 7\[v_1\rightarrow{2a+b+c}\]\[v_2\rightarrow{2a+b+c+d}\]\[v_3\rightarrow{a}\]\[v_4\rightarrow{a+b}\]\[1+2(A)a+(A)b+(A)^2a^{2}+(A)^2ab\]All series and their sums\[\sum_{a\geq{0}}(x_8)^{a}\sum_{b\geq{1}}(x_1)^{b}\sum_{c\geq{0}}(x_2)^{c}\sum_{d\geq{1}}(x_3)^{d}=\frac{(x_1)(x_3)}{(1-x_8)(1-x_1)(1-x_2)(1-x_3)}\]\[2(A)\sum_{a\geq{0}}\textcolor{red}{a}(x_8)^{a}\sum_{b\geq{1}}(x_1)^{b}\sum_{c\geq{0}}(x_2)^{c}\sum_{d\geq{1}}(x_3)^{d}=\frac{2(A)(x_8)(x_1)(x_3)}{(1-x_8)^{\textcolor{red}{2}}(1-x_1)(1-x_2)(1-x_3)}\]\[(A)\sum_{a\geq{0}}(x_8)^{a}\sum_{b\geq{1}}\textcolor{red}{b}(x_1)^{b}\sum_{c\geq{0}}(x_2)^{c}\sum_{d\geq{1}}(x_3)^{d}=\frac{(A)(x_1)(x_3)}{(1-x_8)(1-x_1)^{\textcolor{red}{2}}(1-x_2)(1-x_3)}\]\[(A)^{2}\sum_{a\geq{0}}\textcolor{red}{a^{2}}(x_8)^{a}\sum_{b\geq{1}}(x_1)^{b}\sum_{c\geq{0}}(x_2)^{c}\sum_{d\geq{1}}(x_3)^{d}=\frac{(A^{2})(x^{2}+x_8)(x_1)(x_3)}{(1-x_8)^{\textcolor{red}{3}}(1-x_1)(1-x_2)(1-x_3)}\]\[(A)^{2}\sum_{a\geq{0}}\textcolor{red}{a}(x_8)^{a}\sum_{b\geq{1}}\textcolor{red}{b}(x_1)^{b}\sum_{c\geq{0}}(x_2)^{c}\sum_{d\geq{1}}(x_3)^{d}=\frac{(A^{2})(x_8)(x_1)(x_3)}{(1-x_8)^{\textcolor{red}{2}}(1-x_1)^{\textcolor{red}{2}}(1-x_2)(1-x_3)}\]
Total sum
\[+\frac{(x_1)(x_3)(1-x_8)^{\textcolor{red}{2}}(1-x_1)}{(1-x_8)^{\textcolor{red}{3}}(1-x_1)^{\textcolor{red}{2}}(1-x_2)(1-x_3)}\]\[+\frac{2(A)(x_8)(x_1)(x_3)(1-x_1)(1-x_8)}{(1-x_8)^{\textcolor{red}{3}}(1-x_1)^{\textcolor{red}{2}}(1-x_2)(1-x_3)}\]\[+\frac{(A)(x_1)(x_3)(1-x_8)^{\textcolor{red}{2}}}{(1-x_8)^{\textcolor{red}{3}}(1-x_1)^{\textcolor{red}{2}}(1-x_2)(1-x_3)}\]\[+\frac{(A)^{2}(x^{2}+x_8)(x_1)(x_3)(1-x_1)}{(1-x_8)^{\textcolor{red}{3}}(1-x_1)^{\textcolor{red}{2}}(1-x_2)(1-x_3)}\]\[+\frac{(A)^{2}(x_8)(x_1)(x_3)(1-x_8)}{(1-x_8)^{\textcolor{red}{3}}(1-x_1)^{\textcolor{red}{2}}(1-x_2)(1-x_3)}\]\[x_0\rightarrow{p^{37}t^{20}}\]\[x_1\rightarrow{p^{26}t^{14}}\]\[x_2\rightarrow{p^{18}t^{10}}\]\[x_3\rightarrow{p^{11}t^{6}}\]\[x_4\rightarrow{p^{44}t^{24}}\]\[x_5\rightarrow{p^{7}t^{4}}\]\[x_6\rightarrow{p^{52}t^{28}}\]\[x_7\rightarrow{p^{15}t^{8}}\]\[x_8\rightarrow{p^{55}t^{30}}\]\[x_9\rightarrow{p^{29}t^{16}}\]\[x_10\rightarrow{p^{48}t^{26}}\]\[x_11\rightarrow{p^{63}t^{34}}\]\[x_12\rightarrow{p^{22}t^{12}}\]\end{document}