\documentclass{article}
\usepackage{amsmath}
\usepackage{graphicx} % Required for inserting images
\usepackage{geometry}
 \geometry{
 a4paper,
 total={170mm,257mm},
 left=20mm,
 top=20mm,
 }
\title{v_{11}}
\author{haiml76 }
\date{June 2025}

\begin{document}

%\maketitle

\section{Introduction}
We have the following facts about expressions with $v_{11}$:
\begin{enumerate}
    \item 
$v_{11}\geq{-v_2-\min\{v_1,v_3\}}$
\item $p^{\min\{0,v_2+v_{11}\}}=\left\{
	\begin{array}{ll}
		p^{0}=1  & v_{11}\geq{-v_2} \\
		  p^{-j} & v_{11}=-v_2-j, \text{where\,}j\geq{1}
	\end{array}
\right.$
\item Following from the previous fact, we obtain that

$p^{\min\{0,v_2+v_{11}\}}\mu(a_{11})=\left\{
	\begin{array}{ll}
		p^0p^{v_2}=p^{v_2}  & v_{11}\geq{-v_2} \\
		  p^{-j}(p^{v_2+j}-p^{v_2+j-1)}=p^{v_2}(1-p^{-1}) & v_{11}=-v_2-j, \text{where\,}j\geq{1}
	\end{array}
\right.$
\item $\alpha=\min\{\beta,v_{11}+v_2+\gamma\}$, where $\beta=\min\{v_2,v_4\}$ and $\gamma=\max\{v_1,v_4\}$.
Hence, we have the following settings:
\begin{enumerate}
    \item $\beta=v_2$ and $\gamma=v_1$

$\alpha=\left\{
	\begin{array}{ll}
            v_2  & v_{11}\geq{-v_1} \\
		  v_2-j & v_{11}=-v_1-j, \text{where\,}j\geq{1}
	\end{array}
\right.$    
\item $\beta=v_2$ and $\gamma=v_4$

$\alpha=\left\{
	\begin{array}{ll}
            v_2  & v_{11}\geq{-v_4} \\
		  v_2-j & v_{11}=-v_4-j, \text{where\,}j\geq{1}
	\end{array}
\right.$    
\item $\beta=v_42$ and $\gamma=v_1$

$\alpha=\left\{
	\begin{array}{ll}
            v_4  & v_{11}\geq{v_4-v_1-v_2} \\
		  v_4--j & v_{11}=v_4-v_2-v_1-j, \text{where\,}j\geq{1}
	\end{array}
\right.$    
\item $\beta=v_42$ and $\gamma=v_41$

$\alpha=\left\{
	\begin{array}{ll}
            v_42  & v_{11}\geq{-v_21} \\
		  v_42-j & v_{11}=-v_21-j, \text{where\,}j\geq{1}
	\end{array}
\right.$
\end{enumerate}
\end{enumerate}
\begin{enumerate}
%%%%%%%%%% Case 1 %%%%%%%%%%
    \item $\min\{v_1,v_3\}=v_3$, $\min\{v_2,v_4\}=v_2$, $\max\{v_1,v_4\}=v_1$
    
    \textbf{Constraints}
    \begin{enumerate}
        \item $v_{11}\geq{-v_2-v_3}$
        \item $\alpha=\min\{v_2,v_2+v_{11}+v_1\}$
    \end{enumerate}
    
    \textbf{Sub cases}
    \begin{enumerate}
        \item $v_1\geq{v_2+v_3}\Rightarrow{-v_2-v_3\geq{-v_1}}$

        \begin{enumerate}
            \item $p^{\min\{0,v_2+v_{11}\}}\mu(a_{11})=p^{0}p^{v_2}+\sum_i^{v_3}p^{-i}(p^{v_2+i}-p^{v_2+i-1})=p^{v_2}+\sum_i^{v_3}p^{v_2}(1-p^{-1})=$\[=p^{v_2}(1+v_3(1-p^{-1}))\]
            \item $\alpha=\min\{v_2,v_2+v_{11}+v_1\}$, and $v_{11}>-v_2-v_3\geq{-v_1}\Rightarrow{v_{11}+v_1\geq{0}}\Rightarrow{v_2\leq{v_2+v_{11}+v_1}}\Rightarrow{\alpha=v_2}.$
            \item $\Rightarrow{S=p^{v_2}(1+v_3(1-p^{-1}))(1+v_2(1-p^{-1}))}.$
        \end{enumerate}

        \item $v_1<{v_2+v_3}\Rightarrow{-v_2-v_3<-v_1}$

        \begin{enumerate}
            \item $p^{\min\{0,v_2+v_{11}\}}\mu(a_{11})=
            \left\{
	\begin{array}{ll}
            p^{v_2}(1+(v_1-v_2)(1-p^{-1})) & v_{11}\geq{-v_1} \\
		  p^{v_2}(v_2+v_3-v_1)(1-p^{-1})) & -v_2-v_3\leq{v_{11}}\leq{-v_1-1} \\
	\end{array}
\right.
$
            \item $\alpha=\left\{
	\begin{array}{ll}
            v_2  & v_{11}\geq{-v_1} \\
		  v_2+v_{11}+v_1 & -v_2-v_3\leq{v_{11}}\leq{-v_1-1} \\
	\end{array}
\right.$
        \item $\Rightarrow{S=\left\{
	\begin{array}{ll}
            p^{v_2}(1+(v_1-v_2)(1-p^{-1}))(1+v_2(1-p^{-1}))  & v_{11}\geq{-v_1} \\
		              p^{v_2}[(v_2-(v_1-v_3))(1-p^{-1})+[\binom{v_2}{2}-\binom{v_1-v_3}{2}](1-p^{-1})^2]  & -v_2-v_3\leq{v_{11}}\leq{-v_1-1} \\
	\end{array}
\right.}.$
        \end{enumerate}

    \end{enumerate}
%%%%%%%%%% Case 2 %%%%%%%%%%
    \item $\min\{v_1,v_3\}=v_3$, $\min\{v_2,v_4\}=v_2$, $\max\{v_1,v_4\}=v_4$
    
    \textbf{Constraints}
    \begin{enumerate}
        \item $v_{11}\geq{-v_2-v_3}$
        \item $\alpha=\min\{v_2,v_2+v_{11}+v_4\}$
    \end{enumerate}
    
    \textbf{Sub cases}
    \begin{enumerate}
        \item $v_4\geq{v_2+v_3}\Rightarrow{-v_2-v_3\geq{-v_4}}$

        \begin{enumerate}
            \item $p^{\min\{0,v_2+v_{11}\}}\mu(a_{11})=p^{0}p^{v_2}+\sum_i^{v_3}p^{-i}(p^{v_2+i}-p^{v_2+i-1})=p^{v_2}+\sum_i^{v_3}p^{v_2}(1-p^{-1})=$\[=p^{v_2}(1+v_3(1-p^{-1}))\]
            \item $\alpha=\min\{v_2,v_2+v_{11}+v_4\}$, and $v_{11}>-v_2-v_3\geq{-v_4}\Rightarrow{v_{11}+v_1\geq{0}}\Rightarrow{v_2\leq{v_2+v_{11}+v_4}}\Rightarrow{\alpha=v_2}.$
            \item $\Rightarrow{S=p^{v_2}(1+v_3(1-p^{-1}))(1+v_2(1-p^{-1}))}.$
        \end{enumerate}

        \item $v_4<{v_2+v_3}\Rightarrow{-v_2-v_3<-v_4}$

        \begin{enumerate}
            \item $p^{\min\{0,v_2+v_{11}\}}\mu(a_{11})=
            \left\{
	\begin{array}{ll}
            p^{v_2}(1+(v_4-v_2)(1-p^{-1})) & v_{11}\geq{-v_4} \\
		  p^{v_2}(v_2+v_3-v_4)(1-p^{-1})) & -v_2-v_3\leq{v_{11}}\leq{-v_4-1} \\
	\end{array}
\right.
$
            \item $\alpha=\left\{
	\begin{array}{ll}
            v_2  & v_{11}\geq{-v_4} \\
		  v_2+v_{11}+v_4 & -v_2-v_3\leq{v_{11}}\leq{-v_4-1} \\
	\end{array}
\right.$
        \item $\Rightarrow{S=\left\{
	\begin{array}{ll}
            p^{v_2}(1+(v_4-v_2)(1-p^{-1}))(1+v_2(1-p^{-1}))  & v_{11}\geq{-v_4} \\
		              p^{v_2}[(v_2-(v_4-v_3))(1-p^{-1})+[\binom{v_2}{2}-\binom{v_4-v_3}{2}](1-p^{-1})^2]  & -v_2-v_3\leq{v_{11}}\leq{-v_4-1} \\
	\end{array}
\right.}.$
        \end{enumerate}

    \end{enumerate}

%%%%%%%%%% Case 3 %%%%%%%%%%
    \item $\min\{v_1,v_3\}=v_3$, $\min\{v_2,v_4\}=v_4$, $\max\{v_1,v_4\}=v_1$
    
    \textbf{Constraints}
    \begin{enumerate}
        \item $v_{11}\geq{-v_2-v_3}$
        \item $\alpha=\min\{v_4,v_2+v_{11}+v_1\}$
    \end{enumerate}
    
    \textbf{Sub cases}
    \begin{enumerate}
        \item $v_3\leq{v_1-v_4}\Rightarrow{-v_3\geq{v_4-v_1}}\Rightarrow{-v_2-v_3\geq{v_4-v_1-v_2}}$

        \begin{enumerate}
            \item $p^{\min\{0,v_2+v_{11}\}}\mu(a_{11})=p^{0}p^{v_2}+\sum_i^{v_3}p^{-i}(p^{v_2+i}-p^{v_2+i-1})=p^{v_2}+\sum_i^{v_3}p^{v_2}(1-p^{-1})=$\[=p^{v_2}(1+v_3(1-p^{-1}))\]
            \item $\alpha=\min\{v_4,v_2+v_{11}+v_1\}$, and $v_{11}\geq{-v_2-v_3}\geq{v_4-v_1-v_2}\Rightarrow{v_{11}+v_1+v_2\geq{v_4}}\Rightarrow{\alpha=v_4}.$
            \item $\Rightarrow{S=p^{v_2}(1+v_3(1-p^{-1}))(1+v_4(1-p^{-1}))}.$
        \end{enumerate}

        \item $v_3>{v_1-v_4}\Rightarrow{-v_3<{v_4-v_1}}\Rightarrow{-v_2-v_3<{v_4-v_1-v_2}}$

        \begin{enumerate}
            \item $p^{\min\{0,v_2+v_{11}\}}\mu(a_{11})=
            \left\{
	\begin{array}{ll}
            p^{v_2}(1+(v_1-v_4)(1-p^{-1})) & v_{11}\geq{v_4-v_1-v_2} \\
		  p^{v_2}(v_2+v_3-v_4)(1-p^{-1})) & -v_2-v_3\leq{v_{11}}\leq{v_4-v_1-v_2-1} \\
	\end{array}
\right.
$
            \item $\alpha=\left\{
	\begin{array}{ll}
            v_4  & v_{11}\geq{v_4-v_1-v_2} \\
		  v_4+v_{11}+v_1 & -v_2-v_3\leq{v_{11}}\leq{v_4-v_1-v_2-1} \\
	\end{array}
\right.$
        \item $\Rightarrow{S=\left\{
	\begin{array}{ll}
            p^{v_2}(1+(v_1-v_4)(1-p^{-1}))(1+v_2(1-p^{-1}))  & v_{11}\geq{v_4-v_1-v_2} \\
		              p^{v_2}[(v_2-(v_4-v_3))(1-p^{-1})+[\binom{v_4}{2}-\binom{v_1-v_3}{2}](1-p^{-1})^2]  & -v_2-v_3\leq{v_{11}}\leq{v_4-v_1-v_2-1} \\
	\end{array}
\right.}.$
        \end{enumerate}

    \end{enumerate}

    %%%%%%%%%% Case 4 %%%%%%%%%%
    \item $\min\{v_1,v_3\}=v_3$, $\min\{v_2,v_4\}=v_4$, $\max\{v_1,v_4\}=v_4$
    
    \textbf{Constraints}
    \begin{enumerate}
        \item $v_{11}\geq{-v_2-v_3}$
        \item $\alpha=\min\{v_4,v_2+v_{11}+v_4\}$
    \end{enumerate}
    There are no sub cases here 

        \begin{enumerate}
            \item $p^{\min\{0,v_2+v_{11}\}}\mu(a_{11})=
            \left\{
	\begin{array}{ll}
            p^{0}p^{v_2} & v_{11}\geq{-v_2} \\
		  p^{v_2}(v_3(1-p^{-1})) & -v_2-v_3\leq{v_{11}}\leq{-v_2-1} \\
	\end{array}
\right.
$
            \item $\alpha=\left\{
	\begin{array}{ll}
            v_2  & v_{11}\geq{-v_4} \\
		  v_2+v_{11}+v_4 & -v_2-v_3\leq{v_{11}}\leq{-v_4-1} \\
	\end{array}
\right.$
        \item $\Rightarrow{S=\left\{
	\begin{array}{ll}
            p^{v_2}(1+v_2(1-p^{-1})) & v_{11}\geq{-v_2} \\
		              p^{v_2}[(v_3-(v_1-v_4))(1-p^{-1})+[\binom{v_4}{2}-\binom{v_1-v_3}{2}](1-p^{-1})^2]  & -v_2-v_3\leq{v_{11}}\leq{v_4-v_1-v_2-1} \\
	\end{array}
\right.}.$
        \end{enumerate}
%%%%%%%%%% Case 5 %%%%%%%%%%
    \item $\min\{v_1,v_3\}=v_1$, $\min\{v_2,v_4\}=v_2$, $\max\{v_1,v_4\}=v_1$
    
    \textbf{Constraints}
    \begin{enumerate}
        \item $v_{11}\geq{-v_2-v_1}$
        \item $\alpha=\min\{v_2,v_2+v_{11}+v_1\}$
    \end{enumerate}
There are no sub cases here, because $-v_2-v_1\leq{-v_1}$
        \begin{enumerate}
            \item $p^{\min\{0,v_2+v_{11}\}}\mu(a_{11})=
            \left\{
	\begin{array}{ll}
            p^{v_2}(1+(v_1-v_2)(1-p^{-1})) & v_{11}\geq{-v_1} \\
		  p^{v_2}v_2(1-p^{-1})) & -v_2-v_1\leq{v_{11}}\leq{-v_1-1} \\
	\end{array}
\right.
$
            \item $\alpha=\left\{
	\begin{array}{ll}
            v_2  & v_{11}\geq{-v_1} \\
		  v_2+v_{11}+v_1 & -v_2-v_1\leq{v_{11}}\leq{-v_1-1} \\
	\end{array}
\right.$
        \item $\Rightarrow{S=\left\{
	\begin{array}{ll}
            p^{v_2}(1+(v_1-v_4)(1-p^{-1}))(1+v_2(1-p^{-1}))  & v_{11}\geq{-v_1} \\
		              p^{v_2}[v_2(1-p^{-1})+[\binom{v_2}{2}](1-p^{-1})^2]  & -v_2-v_1\leq{v_{11}}\leq{-v_1-1} \\
	\end{array}
\right.}.$
        \end{enumerate}

        %%%%%%%%%% Case 6 %%%%%%%%%%
    \item $\min\{v_1,v_3\}=v_3$, $\min\{v_2,v_4\}=v_2$, $\max\{v_1,v_4\}=v_4$
    
    \textbf{Constraints}
    \begin{enumerate}
        \item $v_{11}\geq{-v_2-v_1}$
        \item $\alpha=\min\{v_2,v_2+v_{11}+v_4\}$
    \end{enumerate}
    
    \textbf{Sub cases}
    \begin{enumerate}
        \item $v_2+v_1\leq{v_4}\Rightarrow{-v_2-v_1\geq{-v_4}}$

        \begin{enumerate}
            \item $p^{\min\{0,v_2+v_{11}\}}\mu(a_{11})=p^{0}p^{v_2}+\sum_i^{v_1}p^{-i}(p^{v_2+i}-p^{v_2+i-1})=p^{v_2}+\sum_i^{v_1}p^{v_2}(1-p^{-1})=$\[=p^{v_2}(1+v_1(1-p^{-1}))\]
            \item $\alpha=\min\{v_2,v_2+v_{11}+v_4\}$, and $v_{11}\geq{-v_2-v_1}\geq{-v_4}\Rightarrow{v_{11}+v_4+v_2\geq{v_2}}\Rightarrow{\alpha=v_2}.$
            \item $\Rightarrow{S=p^{v_2}(1+v_1(1-p^{-1}))(1+v_2(1-p^{-1}))}.$
        \end{enumerate}

        \item $v_2+v_1>{v_4}\Rightarrow{-v_4>{-v_2-v_1}}$

        \begin{enumerate}
            \item $p^{\min\{0,v_2+v_{11}\}}\mu(a_{11})=
            \left\{
	\begin{array}{ll}
            p^{v_2}(1+(v_4-v_2)(1-p^{-1})) & v_{11}\geq{-v_4} \\
		  p^{v_2}(v_2+v_1-v_4)(1-p^{-1})) & -v_2-v_1\leq{v_{11}}\leq{-v_4-1} \\
	\end{array}
\right.
$
            \item $\alpha=\left\{
	\begin{array}{ll}
            v_2  & v_{11}\geq{-v_4} \\
		  v_2+v_{11}+v_4 & -v_2-v_1\leq{v_{11}}\leq{v_4-v_1} \\
	\end{array}
\right.$
        \item $\Rightarrow{S=\left\{
	\begin{array}{ll}
            p^{v_2}(1+(v_4-v_2)(1-p^{-1}))(1+v_2(1-p^{-1}))  & v_{11}\geq{v_4-v_1-v_2} \\
		              p^{v_2}[(v_2-(v_4-v_3))(1-p^{-1})+[\binom{v_2}{2}-\binom{v_4-v_1}{2}](1-p^{-1})^2]  & -v_2-v_1\leq{v_{11}}\leq{-v_4-1} \\
	\end{array}
\right.}.$
        \end{enumerate}

    \end{enumerate}

    %%%%%%%%%% Case 7 %%%%%%%%%%
    \item $\min\{v_1,v_3\}=v_1$, $\min\{v_2,v_4\}=v_4$, $\max\{v_1,v_4\}=v_1$
    
    \textbf{Constraints}
    \begin{enumerate}
        \item $v_{11}\geq{-v_2-v_1}$
        \item $\alpha=\min\{v_4,v_2+v_{11}+v_1\}$
    \end{enumerate}
There are no sub cases here, because $-v_2-v_1\leq{v_4-v_2-v_1}$
        \begin{enumerate}
            \item $p^{\min\{0,v_2+v_{11}\}}\mu(a_{11})=
            \left\{
	\begin{array}{ll}
            p^{v_2}(1+(v_1-v_4)(1-p^{-1})) & v_{11}\geq{v_4-v_2-v_1} \\
		  p^{v_2}v_4(1-p^{-1})) & -v_2-v_1\leq{v_{11}}\leq{v_4-v_2-v_1-1} \\
	\end{array}
\right.
$
            \item $\alpha=\left\{
	\begin{array}{ll}
            v_4  & v_{11}\geq{v_4-v_2-v_1} \\
		  v_2+v_{11}+v_1 & -v_2-v_1\leq{v_{11}}\leq{v_4-v_2-v_1-1} \\
	\end{array}
\right.$
        \item $\Rightarrow{S=\left\{
	\begin{array}{ll}
            p^{v_2}(1+(v_1-v_4)(1-p^{-1}))(1+v_4(1-p^{-1}))  & v_{11}\geq{v_4-v_2-v_1} \\
		              p^{v_2}[v_4(1-p^{-1})+[\binom{v_4}{2}](1-p^{-1})^2]  & -v_2-v_1\leq{v_{11}}\leq{v_4-v_2-v_1-1} \\
	\end{array}
\right.}.$
        \end{enumerate}
    \end{enumerate}
\end{document}
